Impl/InsertModel.i.dfy
@@ -7,6 +7,9 @@ module InsertModel {
   import opened BookkeepingModel
   import opened FlushPolicyModel
   import opened NodeModel
+  import opened InterpretationDiskOps
+  import opened ViewOp
+  import opened DiskOpModel
 
   import opened Options
   import opened Maps
@@ -24,9 +27,9 @@ module InsertModel {
 
   // == insert ==
 
-  function {:opaque} InsertKeyValue(k: Constants, s: Variables, key: Key, value: Value)
-  : (Variables, bool)
-  requires Inv(k, s)
+  function {:opaque} InsertKeyValue(k: Constants, s: BCVariables, key: Key, value: Value)
+  : (BCVariables, bool)
+  requires BCInv(k, s)
   requires s.Ready?
   requires BT.G.Root() in s.cache
   requires |s.ephemeralIndirectionTable.graph| <= IndirectionTableModel.MaxSize() - 1
@@ -48,8 +51,8 @@ module InsertModel {
     )
   }
 
-  lemma InsertKeyValueCorrect(k: Constants, s: Variables, key: Key, value: Value)
-  requires Inv(k, s)
+  lemma InsertKeyValueCorrect(k: Constants, s: BCVariables, key: Key, value: Value, replay: bool)
+  requires BCInv(k, s)
   requires s.Ready?
   requires BT.G.Root() in s.cache
   requires |s.ephemeralIndirectionTable.graph| <= IndirectionTableModel.MaxSize() - 1
@@ -57,8 +60,15 @@ module InsertModel {
       WeightBucketList(s.cache[BT.G.Root()].buckets) 
       <= MaxTotalBucketWeight()
   ensures var (s', success) := InsertKeyValue(k, s, key, value);
-      && WFVars(s')
-      && M.Next(Ik(k), IVars(s), IVars(s'), if success then UI.PutOp(key, value) else UI.NoOp, D.NoDiskOp)
+      && WFBCVars(s')
+      && (success ==>
+        BBC.Next(Ik(k).bc, IBlockCache(s), IBlockCache(s'),
+          BlockDisk.NoDiskOp,
+          AdvanceOp(UI.PutOp(key, value), replay))
+      )
+      && (!success ==>
+        betree_next(k, IBlockCache(s), IBlockCache(s'))
+      )
   {
     reveal_InsertKeyValue();
     reveal_CacheInsertKeyValue();
@@ -70,7 +80,7 @@ module InsertModel {
       assert (s.frozenIndirectionTable.Some? && BT.G.Root() in IIndirectionTable(s.frozenIndirectionTable.value).graph) &&
           !(BT.G.Root() in IIndirectionTable(s.frozenIndirectionTable.value).locs);
       // TODO write out the root here instead of giving up
-      assert noop(k, IVars(s), IVars(s));
+      assert noop(k, IBlockCache(s), IBlockCache(s));
       return;
     }
 
@@ -107,35 +117,30 @@ module InsertModel {
     assert BT.ValidInsertion(BT.MessageInsertion(key, msg, oldroot));
 
     assert WFNode(newRoot);
-    assert WFVars(s');
+    assert WFBCVars(s');
 
-    assert BC.Dirty(Ik(k), IVars(s), IVars(s'), BT.G.Root(), newroot);
-    assert BC.OpStep(Ik(k), IVars(s), IVars(s'), BT.G.WriteOp(BT.G.Root(), newroot));
+    assert BC.Dirty(Ik(k).bc, IBlockCache(s), IBlockCache(s'), BT.G.Root(), newroot);
+    assert BC.OpStep(Ik(k).bc, IBlockCache(s), IBlockCache(s'), BT.G.WriteOp(BT.G.Root(), newroot));
     assert BT.ValidBetreeStep(btStep);
-    assert BC.OpStep(Ik(k), IVars(s), IVars(s'), BT.BetreeStepOps(btStep)[0]);
-    assert BC.OpTransaction(Ik(k), IVars(s), IVars(s'), BT.BetreeStepOps(btStep));
-    assert BBC.BetreeMove(Ik(k), IVars(s), IVars(s'), UI.PutOp(key, value), SD.NoDiskOp, btStep);
-    assert stepsBetree(k, IVars(s), IVars(s'), UI.PutOp(key, value), btStep);
-
-    assert M.NextStep(Ik(k), IVars(s), IVars(s'), UI.PutOp(key, value), D.NoDiskOp,
-        M.Step(BBC.BetreeMoveStep(btStep)));
+    assert BC.OpStep(Ik(k).bc, IBlockCache(s), IBlockCache(s'), BT.BetreeStepOps(btStep)[0]);
+    assert BC.OpTransaction(Ik(k).bc, IBlockCache(s), IBlockCache(s'), BT.BetreeStepOps(btStep));
+    assert BBC.BetreeMove(Ik(k).bc, IBlockCache(s), IBlockCache(s'), BlockDisk.NoDiskOp, AdvanceOp(UI.PutOp(key, value), replay), btStep);
+    assert stepsBetree(k, IBlockCache(s), IBlockCache(s'), AdvanceOp(UI.PutOp(key, value), replay), btStep);
   }
 
-  predicate {:opaque} insert(k: Constants, s: Variables, io: IO, key: Key, value: Value,
-      s': Variables, success: bool, io': IO)
+  predicate {:opaque} insert(k: Constants, s: BCVariables, io: IO, key: Key, value: Value,
+      s': BCVariables, success: bool, io': IO)
   requires io.IOInit?
-  requires Inv(k, s)
+  requires s.Ready?
+  requires BCInv(k, s)
   {
-    if (s.Unready?) then (
-      && (s', io') == PageInIndirectionTableReq(k, s, io)
-      && success == false
-    ) else if !(|s.ephemeralIndirectionTable.graph| <= IndirectionTableModel.MaxSize() - 3) then (
+    if !(|s.ephemeralIndirectionTable.graph| <= IndirectionTableModel.MaxSize() - 3) then (
       && s' == s
       && io' == io
       && success == false
     ) else if (BT.G.Root() !in s.cache) then (
       if TotalCacheSize(s) <= MaxCacheSize() - 1 then (
-        && (s', io') == PageInReq(k, s, io, BT.G.Root())
+        && (s', io') == PageInNodeReq(k, s, io, BT.G.Root())
         && success == false
       ) else (
         // TODO rule out this case?
@@ -154,35 +159,39 @@ module InsertModel {
     )
   }
 
-  lemma insertCorrect(k: Constants, s: Variables, io: IO, key: Key, value: Value,
-      s': Variables, success: bool, io': IO)
+  lemma insertCorrect(k: Constants, s: BCVariables, io: IO, key: Key, value: Value,
+      s': BCVariables, success: bool, io': IO, replay: bool)
   requires io.IOInit?
-  requires Inv(k, s)
+  requires s.Ready?
+  requires BCInv(k, s)
   requires insert(k, s, io, key, value, s', success, io');
-  ensures WFVars(s')
-  ensures M.Next(Ik(k), IVars(s), IVars(s'),
-        if success then UI.PutOp(key, value) else UI.NoOp,
-        diskOp(io'))
+  ensures WFBCVars(s')
+  ensures ValidDiskOp(diskOp(io'))
+  ensures IDiskOp(diskOp(io')).jdop.NoDiskOp?
+
+  ensures success ==>
+        BBC.Next(Ik(k).bc, IBlockCache(s), IBlockCache(s'),
+          IDiskOp(diskOp(io')).bdop,
+          AdvanceOp(UI.PutOp(key, value), replay))
+  ensures !success ==>
+        betree_next_dop(k, IBlockCache(s), IBlockCache(s'), IDiskOp(diskOp(io')).bdop)
   {
     reveal_insert();
 
-    if (s.Unready?) {
-      PageInIndirectionTableReqCorrect(k, s, io);
-    } else if !(|s.ephemeralIndirectionTable.graph| <= IndirectionTableModel.MaxSize() - 3) {
-      assert noop(k, IVars(s), IVars(s));
+    if !(|s.ephemeralIndirectionTable.graph| <= IndirectionTableModel.MaxSize() - 3) {
+      assert noop(k, IBlockCache(s), IBlockCache(s));
     } else if (BT.G.Root() !in s.cache) {
       if TotalCacheSize(s) <= MaxCacheSize() - 1 {
-        PageInReqCorrect(k, s, io, BT.G.Root());
+        PageInNodeReqCorrect(k, s, io, BT.G.Root());
       } else {
-        assert noop(k, IVars(s), IVars(s));
+        assert noop(k, IBlockCache(s), IBlockCache(s));
       }
     } else if WeightKey(key) + WeightMessage(Messages.Define(value)) +
         WeightBucketList(s.cache[BT.G.Root()].buckets) 
         <= MaxTotalBucketWeight() {
-      InsertKeyValueCorrect(k, s, key, value);
+      InsertKeyValueCorrect(k, s, key, value, replay);
     } else {
       runFlushPolicyCorrect(k, s, io, s', io');
     }
   }
-
 }
