Impl/MainHandlers.i.dfy
@@ -1,75 +1,76 @@
 include "Main.s.dfy"
 include "../lib/Base/Sets.i.dfy"
-include "../ByteBlockCacheSystem/ByteBetreeBlockCacheSystem.i.dfy"
-include "../ByteBlockCacheSystem/Marshalling.i.dfy"
-include "InsertImpl.i.dfy"
-include "QueryImpl.i.dfy"
-include "SuccImpl.i.dfy"
-include "InsertModel.i.dfy"
-include "QueryModel.i.dfy"
-include "SyncModel.i.dfy"
+include "CoordinationImpl.i.dfy"
+include "HandleReadResponseImpl.i.dfy"
+include "HandleWriteResponseImpl.i.dfy"
 include "Mkfs.i.dfy"
-include "../ByteBlockCacheSystem/ByteBetreeBlockCacheSystem_Refines_ThreeStateVersionedMap.i.dfy"
+include "CoordinationModel.i.dfy"
+include "../ByteBlockCacheSystem/ByteSystem_Refines_ThreeStateVersionedMap.i.dfy"
+
 //
 // Implements the application-API-handler obligations laid out by Main.s.dfy. TODO rename in a way that emphasizes that this is a module-refinement of the abstract Main that satisfies its obligations.
 //
 
 module {:extern} MainHandlers refines Main { 
+  import DOM = DiskOpModel
   import SM = StateModel
   import SI = StateImpl
-  import IOImpl
-  import opened InsertImpl
-  import opened QueryImpl
-  import opened SyncImpl
-  import opened SuccImpl
-  import IOModel
-  import InsertModel
-  import QueryModel
-  import SyncModel
-  import SuccModel
+  import CoordinationImpl
+  import HandleReadResponseImpl
+  import HandleReadResponseModel
+  import HandleWriteResponseImpl
+  import HandleWriteResponseModel
+  import CoordinationModel
+  import FullImpl
   import MkfsImpl
   import MkfsModel
 
-  import BBC = BetreeBlockCache
-  import BC = BetreeGraphBlockCache
-  import ADM = ByteBetreeBlockCacheSystem
+  import BlockJournalCache
+  import BBC = BetreeCache
+  import BC = BlockCache
+  import JC = JournalCache
+  import ADM = ByteSystem
 
-  import System_Ref = ByteBetreeBlockCacheSystem_Refines_ThreeStateVersionedMap
+  import opened DiskOpImpl
+  import opened InterpretationDiskOps
 
-  type Constants = SI.ImplConstants
-  type Variables = SI.ImplVariables
+  import System_Ref = ByteSystem_Refines_ThreeStateVersionedMap
+
+  type Constants = ImplConstants
+  type Variables = FullImpl.Full
 
   function HeapSet(hs: HeapState) : set<object> { hs.Repr }
 
   predicate Inv(k: Constants, hs: HeapState)
   {
-    // TODO this is gross, what can we do about it?
     && hs.s in HeapSet(hs)
-    && (
-        {hs.s.persistentIndirectionTable, hs.s.ephemeralIndirectionTable, hs.s.lru, hs.s.cache, hs.s.blockAllocator, hs.s.syncReqs} +
-        (if hs.s.frozenIndirectionTable != null then {hs.s.frozenIndirectionTable} else {})
-       ) <= HeapSet(hs)
-    && hs.s.Repr() <= HeapSet(hs)
-    && SI.Inv(k, hs.s)
+    && hs.s.Repr <= HeapSet(hs)
+    && hs.s.Inv(k)
   }
 
-  function Ik(k: Constants) : ADM.M.Constants { BC.Constants() }
-  function I(k: Constants, hs: HeapState) : ADM.M.Variables { SM.IVars(hs.s.I()) }
+  function Ik(k: Constants) : ADM.M.Constants {
+    BlockJournalCache.Constants(BC.Constants(), JC.Constants())
+  }
+  function I(k: Constants, hs: HeapState) : ADM.M.Variables {
+    SM.IVars(hs.s.I())
+  }
 
   method InitState() returns (k: Constants, hs: HeapState)
+    // conditions inherited:
+    //ensures Inv(k, hs)
+    //ensures ADM.M.Init(Ik(k), I(k, hs))
   {
-    k := BC.Constants();
-    var s := new Variables();
+    var s := new Variables(k);
     hs := new HeapState(s, {});
-    hs.Repr := s.Repr() + {s};
+    hs.Repr := s.Repr + {s};
     assert Inv(k, hs);
-    BBC.InitImpliesInv(Ik(k), I(k, hs));
+    BlockJournalCache.InitImpliesInv(Ik(k), I(k, hs));
   }
 
   lemma ioAndHsNotInReadSet(s: Variables, io: DiskIOHandler, hs: HeapState)
   requires s.W()
-  ensures io !in s.Repr()
-  ensures hs !in s.Repr()
+  ensures io !in s.Repr
+  ensures hs !in s.Repr
   // TODO I think this should just follow from the types of the objects
   // in the Repr
 
@@ -80,29 +81,42 @@ module {:extern} MainHandlers refines Main {
   {
     var s := hs.s;
     ioAndHsNotInReadSet(s, io, hs);
-    SyncModel.pushSyncCorrect(SI.Ic(k), s.I());
-    var id1 := pushSync(k, s);
+    var id1 := CoordinationImpl.pushSync(k, s);
+
+    CoordinationModel.pushSyncCorrect(Ic(k), old(s.I()));
+
+    //assert ADM.M.Next(DOM.Ik(Ic(k)), SM.IVars(old(s.I())), SM.IVars(s.I()),
+    //   if id1 == 0 then UI.NoOp else UI.PushSyncOp(id1 as int),
+    //   D.NoDiskOp);
+
     ioAndHsNotInReadSet(s, io, hs);
     id := id1;
     ghost var uiop := if id == 0 then UI.NoOp else UI.PushSyncOp(id as int);
-    BBC.NextPreservesInv(k, SM.IVars(old(s.I())), SM.IVars(s.I()), uiop, ADM.M.IDiskOp(io.diskOp()));
-    hs.Repr := s.Repr() + {s};
+    if ValidDiskOp(io.diskOp()) {
+      BlockJournalCache.NextPreservesInv(DOM.Ik(Ic(k)), SM.IVars(old(s.I())), SM.IVars(s.I()), uiop, IDiskOp(io.diskOp()));
+    }
+    hs.Repr := s.Repr + {s};
+    //assert SM.Inv(Ic(k), hs.s.I());
+    //assert hs.s.Inv(k);
+    //assert Inv(k, hs);
     assert ADM.M.Next(Ik(k), old(I(k, hs)), I(k, hs), uiop, io.diskOp()); // observe
   }
 
-  method handlePopSync(k: Constants, hs: HeapState, io: DiskIOHandler, id: uint64)
+  method handlePopSync(k: Constants, hs: HeapState, io: DiskIOHandler, id: uint64, graphSync: bool)
   returns (wait: bool, success: bool)
   {
     var s := hs.s;
     ioAndHsNotInReadSet(s, io, hs);
-    var w, succ := popSync(k, s, io, id);
-    SyncModel.popSyncCorrect(SI.Ic(k), old(s.I()), old(SI.IIO(io)), id, s.I(), succ, SI.IIO(io));
+    var succ, w := CoordinationImpl.popSync(k, s, io, id, graphSync);
+    CoordinationModel.popSyncCorrect(Ic(k), old(s.I()), old(IIO(io)), id, graphSync, s.I(), IIO(io), succ);
     ioAndHsNotInReadSet(s, io, hs);
     success := succ;
     wait := w;
     ghost var uiop := if succ then UI.PopSyncOp(id as int) else UI.NoOp;
-    BBC.NextPreservesInv(k, SM.IVars(old(s.I())), SM.IVars(s.I()), uiop, ADM.M.IDiskOp(io.diskOp()));
-    hs.Repr := s.Repr() + {s};
+    if ValidDiskOp(io.diskOp()) {
+      BlockJournalCache.NextPreservesInv(DOM.Ik(Ic(k)), SM.IVars(old(s.I())), SM.IVars(s.I()), uiop, IDiskOp(io.diskOp()));
+    }
+    hs.Repr := s.Repr + {s};
     assert ADM.M.Next(Ik(k), old(I(k, hs)), I(k, hs), // observe
         uiop,
         io.diskOp());
@@ -113,12 +127,14 @@ module {:extern} MainHandlers refines Main {
   {
     var s := hs.s;
     ioAndHsNotInReadSet(s, io, hs);
-    var value := query(k, s, io, key);
-    QueryModel.queryCorrect(SI.Ic(k), old(s.I()), old(SI.IIO(io)), key, s.I(), value, SI.IIO(io));
+    var value := CoordinationImpl.query(k, s, io, key);
+    CoordinationModel.queryCorrect(Ic(k), old(s.I()), old(IIO(io)), key, s.I(), value, IIO(io));
     ioAndHsNotInReadSet(s, io, hs);
     ghost var uiop := if value.Some? then UI.GetOp(key, value.value) else UI.NoOp;
-    BBC.NextPreservesInv(k, SM.IVars(old(s.I())), SM.IVars(s.I()), uiop, ADM.M.IDiskOp(io.diskOp()));
-    hs.Repr := s.Repr() + {s};
+    if ValidDiskOp(io.diskOp()) {
+      BlockJournalCache.NextPreservesInv(DOM.Ik(Ic(k)), SM.IVars(old(s.I())), SM.IVars(s.I()), uiop, IDiskOp(io.diskOp()));
+    }
+    hs.Repr := s.Repr + {s};
     v := value;
     assert ADM.M.Next(Ik(k), old(I(k, hs)), I(k, hs), // observe
         if v.Some? then UI.GetOp(key, v.value) else UI.NoOp,
@@ -130,12 +146,14 @@ module {:extern} MainHandlers refines Main {
   {
     var s := hs.s;
     ioAndHsNotInReadSet(s, io, hs);
-    var succ := insert(k, s, io, key, value);
-    InsertModel.insertCorrect(SI.Ic(k), old(s.I()), old(SI.IIO(io)), key, value, s.I(), succ, SI.IIO(io));
+    var succ := CoordinationImpl.insert(k, s, io, key, value);
+    CoordinationModel.insertCorrect(Ic(k), old(s.I()), old(IIO(io)), key, value, s.I(), succ, IIO(io));
     ioAndHsNotInReadSet(s, io, hs);
     ghost var uiop := if succ then UI.PutOp(key, value) else UI.NoOp;
-    BBC.NextPreservesInv(k, SM.IVars(old(s.I())), SM.IVars(s.I()), uiop, ADM.M.IDiskOp(io.diskOp()));
-    hs.Repr := s.Repr() + {s};
+    if ValidDiskOp(io.diskOp()) {
+      BlockJournalCache.NextPreservesInv(DOM.Ik(Ic(k)), SM.IVars(old(s.I())), SM.IVars(s.I()), uiop, IDiskOp(io.diskOp()));
+    }
+    hs.Repr := s.Repr + {s};
     success := succ;
     assert ADM.M.Next(Ik(k), old(I(k, hs)), I(k, hs), // observe
         if success then UI.PutOp(key, value) else UI.NoOp,
@@ -147,13 +165,15 @@ module {:extern} MainHandlers refines Main {
   {
     var s := hs.s;
     ioAndHsNotInReadSet(s, io, hs);
-    var value := doSucc(k, s, io, start, maxToFind);
-    SuccModel.doSuccCorrect(SI.Ic(k), old(s.I()), old(SI.IIO(io)), start, maxToFind as int);
+    var value := CoordinationImpl.succ(k, s, io, start, maxToFind);
+    CoordinationModel.succCorrect(Ic(k), old(s.I()), old(IIO(io)), start, maxToFind as int, s.I(), value, IIO(io));
     ioAndHsNotInReadSet(s, io, hs);
     ghost var uiop := 
       if value.Some? then UI.SuccOp(start, value.value.results, value.value.end) else UI.NoOp;
-    BBC.NextPreservesInv(k, SM.IVars(old(s.I())), SM.IVars(s.I()), uiop, ADM.M.IDiskOp(io.diskOp()));
-    hs.Repr := s.Repr() + {s};
+    if ValidDiskOp(io.diskOp()) {
+      BlockJournalCache.NextPreservesInv(DOM.Ik(Ic(k)), SM.IVars(old(s.I())), SM.IVars(s.I()), uiop, IDiskOp(io.diskOp()));
+    }
+    hs.Repr := s.Repr + {s};
     res := value;
     assert ADM.M.Next(Ik(k), old(I(k, hs)), I(k, hs), // observe
         uiop,
@@ -164,12 +184,14 @@ module {:extern} MainHandlers refines Main {
   {
     var s := hs.s;
     ioAndHsNotInReadSet(s, io, hs);
-    IOImpl.readResponse(k, s, io);
-    IOModel.readResponseCorrect(SI.Ic(k), old(s.I()), old(SI.IIO(io)));
+    HandleReadResponseImpl.readResponse(k, s, io);
+    HandleReadResponseModel.readResponseCorrect(Ic(k), old(s.I()), old(IIO(io)));
     ioAndHsNotInReadSet(s, io, hs);
     ghost var uiop := UI.NoOp;
-    BBC.NextPreservesInv(k, SM.IVars(old(s.I())), SM.IVars(s.I()), uiop, ADM.M.IDiskOp(io.diskOp()));
-    hs.Repr := s.Repr() + {s};
+    if ValidDiskOp(io.diskOp()) {
+      BlockJournalCache.NextPreservesInv(DOM.Ik(Ic(k)), SM.IVars(old(s.I())), SM.IVars(s.I()), uiop, IDiskOp(io.diskOp()));
+    }
+    hs.Repr := s.Repr + {s};
     assert ADM.M.Next(Ik(k), old(I(k, hs)), I(k, hs), UI.NoOp, io.diskOp()); // observe
   }
 
@@ -177,12 +199,14 @@ module {:extern} MainHandlers refines Main {
   {
     var s := hs.s;
     ioAndHsNotInReadSet(s, io, hs);
-    IOImpl.writeResponse(k, s, io);
-    IOModel.writeResponseCorrect(SI.Ic(k), old(s.I()), old(SI.IIO(io)));
+    HandleWriteResponseImpl.writeResponse(k, s, io);
+    HandleWriteResponseModel.writeResponseCorrect(Ic(k), old(s.I()), old(IIO(io)));
     ioAndHsNotInReadSet(s, io, hs);
     ghost var uiop := UI.NoOp;
-    BBC.NextPreservesInv(k, SM.IVars(old(s.I())), SM.IVars(s.I()), uiop, ADM.M.IDiskOp(io.diskOp()));
-    hs.Repr := s.Repr() + {s};
+    if ValidDiskOp(io.diskOp()) {
+      BlockJournalCache.NextPreservesInv(DOM.Ik(Ic(k)), SM.IVars(old(s.I())), SM.IVars(s.I()), uiop, IDiskOp(io.diskOp()));
+    }
+    hs.Repr := s.Repr + {s};
     assert ADM.M.Next(Ik(k), old(I(k, hs)), I(k, hs), UI.NoOp, io.diskOp()); // observe
   }
 
