BlockCacheSystem/BetreeSystem.i.dfy
@@ -1,0 +1,249 @@
+include "BlockDisk.i.dfy"
+include "../PivotBetree/PivotBetree_Refines_Betree.i.dfy"
+include "../lib/Base/Maps.s.dfy"
+include "../lib/Base/sequences.i.dfy"
+include "BlockSystem.i.dfy"
+include "BetreeCache.i.dfy"
+include "../BlockCacheSystem/BlockSystem_Refines_StatesView.i.dfy"
+//
+// Instantiate the {PivotBetree, BlockCache} code in a System (model of the environment).
+// ("Bottom lettuce")
+//
+
+// TODO(jonh): Rename PivotBetreeBlockCacheSystem. [approved by thance]
+
+module BetreeSystem {
+  import D = BlockDisk
+  import M = BetreeCache
+  import AsyncSectorDiskModelTypes
+  import opened SectorType
+  import opened ViewOp
+  import opened DiskLayout
+  import opened Maps
+  import opened Sequences
+  import opened Options
+
+  import opened PivotBetreeSpec`Spec
+  import BC = BlockCache
+  import BCS = BlockSystem
+  import BT = PivotBetree
+  import BI = PivotBetreeBlockInterface
+  import Ref = BlockSystem_Refines_StatesView
+
+  type Constants = AsyncSectorDiskModelTypes.AsyncSectorDiskModelConstants<M.Constants, D.Constants>
+  type Variables = AsyncSectorDiskModelTypes.AsyncSectorDiskModelVariables<M.Variables, D.Variables>
+
+  datatype Step =
+    | MachineStep(dop: D.DiskOp)
+    | CrashStep
+  
+  predicate Machine(k: Constants, s: Variables, s': Variables, dop: D.DiskOp, vop: VOp)
+  {
+    && M.Next(k.machine, s.machine, s'.machine, dop, vop)
+    && D.Next(k.disk, s.disk, s'.disk, dop)
+    && (vop.SendPersistentLocOp? ==>
+      BCS.Inv(k, s) ==>
+        && vop.loc in Ref.DiskGraphMap(k, s)
+        && BT.Inv(Ik(k), BT.Variables(BI.Variables(Ref.DiskGraphMap(k, s)[vop.loc])))
+    )
+  }
+
+  predicate Crash(k: Constants, s: Variables, s': Variables, vop: VOp)
+  {
+    && vop.CrashOp?
+    && M.Init(k.machine, s'.machine)
+    && D.Crash(k.disk, s.disk, s'.disk)
+  }
+
+  predicate NextStep(k: Constants, s: Variables, s': Variables, vop: VOp, step: Step)
+  {
+    match step {
+      case MachineStep(dop) => Machine(k, s, s', dop, vop)
+      case CrashStep => Crash(k, s, s', vop)
+    }
+  }
+
+  predicate Next(k: Constants, s: Variables, s': Variables, vop: VOp) {
+    exists step :: NextStep(k, s, s', vop, step)
+  }
+
+  function Ik(k: Constants) : BT.Constants
+  {
+    BT.Constants(BI.Constants())
+  }
+
+  function BetreeDisk(k: Constants, s: Variables) : imap<Location, BT.Variables>
+  requires BCS.Inv(k, s)
+  {
+    imap loc | loc in Ref.DiskGraphMap(k, s) ::
+      BT.Variables(BI.Variables(Ref.DiskGraphMap(k, s)[loc]))
+  }
+
+  function FrozenBetree(k: Constants, s: Variables) : Option<BT.Variables>
+  requires BCS.Inv(k, s)
+  {
+    if Ref.FrozenGraph(k, s).Some? then
+      Some(BT.Variables(BI.Variables(Ref.FrozenGraph(k, s).value)))
+    else
+      None
+  }
+
+  function EphemeralBetree(k: Constants, s: Variables) : Option<BT.Variables>
+  requires BCS.Inv(k, s)
+  {
+    if Ref.EphemeralGraph(k, s).Some? then
+      Some(BT.Variables(BI.Variables(Ref.EphemeralGraph(k, s).value)))
+    else
+      None
+  }
+
+  predicate Init(k: Constants, s: Variables, loc: Location)
+  {
+    && M.Init(k.machine, s.machine)
+    && D.Init(k.disk, s.disk)
+    && BCS.Init(k, s, loc)
+    && (
+      BCS.InitImpliesInv(k, s, loc);
+      && loc in BetreeDisk(k, s)
+      && BT.Init(Ik(k), BetreeDisk(k, s)[loc])
+    )
+  }
+
+  predicate Inv(k: Constants, s: Variables) {
+    && BCS.Inv(k, s)
+    && (Ref.PersistentLoc(k, s).Some? ==>
+      && Ref.PersistentLoc(k, s).value in BetreeDisk(k, s)
+      && BT.Inv(Ik(k), BetreeDisk(k, s)[Ref.PersistentLoc(k, s).value])
+    )
+    && (FrozenBetree(k, s).Some? ==> BT.Inv(Ik(k), FrozenBetree(k, s).value))
+    && (EphemeralBetree(k, s).Some? ==> BT.Inv(Ik(k), EphemeralBetree(k, s).value))
+    && (Ref.FrozenLoc(k, s).Some? ==>
+      && Ref.FrozenLoc(k, s).value in BetreeDisk(k, s)
+      && FrozenBetree(k, s).Some?
+      && BetreeDisk(k, s)[Ref.FrozenLoc(k, s).value] == FrozenBetree(k, s).value
+    )
+  }
+
+  // Proofs
+
+  lemma InitImpliesInv(k: Constants, s: Variables, loc: Location)
+    requires Init(k, s, loc)
+    ensures Inv(k, s)
+    ensures loc in BetreeDisk(k, s)
+  {
+    BCS.InitImpliesInv(k, s, loc);
+    BT.InitImpliesInv(Ik(k), BetreeDisk(k, s)[loc]);
+    BCS.InitGraphs(k, s, loc);
+  }
+
+  lemma BetreeMoveStepPreservesInv(k: Constants, s: Variables, s': Variables, dop: D.DiskOp, vop: VOp, betreeStep: BetreeStep)
+    requires Inv(k, s)
+    requires M.BetreeMove(k.machine, s.machine, s'.machine, dop, vop, betreeStep)
+    requires D.Next(k.disk, s.disk, s'.disk, dop)
+    ensures Inv(k, s')
+  {
+    Ref.StepGraphs(k, s, s', vop, BCS.MachineStep(dop, BC.TransactionStep(BetreeStepOps(betreeStep))));
+    Ref.RefinesReads(k, s, BetreeStepReads(betreeStep));
+    //assert BT.Betree(Ik(k), EphemeralBetree(k, s), EphemeralBetree(k, s'), uiop, betreeStep);
+    assert BT.NextStep(Ik(k), EphemeralBetree(k, s).value, EphemeralBetree(k, s').value, vop.uiop, BT.BetreeStep(betreeStep));
+    BT.NextPreservesInv(Ik(k), EphemeralBetree(k, s).value, EphemeralBetree(k, s').value, vop.uiop);
+  }
+
+  lemma BlockCacheMoveStepPreservesInv(k: Constants, s: Variables, s': Variables, dop: D.DiskOp, vop: VOp, step: BC.Step)
+    requires Inv(k, s)
+    requires !step.TransactionStep?
+    requires M.BlockCacheMove(k.machine, s.machine, s'.machine, dop, vop, step)
+    requires D.Next(k.disk, s.disk, s'.disk, dop)
+    requires (vop.SendPersistentLocOp? ==>
+      && vop.loc in BetreeDisk(k, s)
+      && BT.Inv(Ik(k), BetreeDisk(k, s)[vop.loc])
+    )
+    ensures Inv(k, s')
+  {
+    assert BCS.Machine(k, s, s', dop, vop, step);
+    Ref.StepGraphs(k, s, s', vop, BCS.MachineStep(dop, step));
+    if (step.UnallocStep?) {
+      //assert BI.GC(Ik(k).bck, EphemeralBetree(k, s).bcv, s'.bcv, refs)
+      Ref.UnallocStepMeetsGCConditions(k, s, s', dop, vop, step.ref);
+      assert step.ref in EphemeralBetree(k, s).value.bcv.view;
+      assert iset{step.ref} !! BI.LiveReferences(Ik(k).bck, EphemeralBetree(k, s).value.bcv);
+      assert BI.ClosedUnderPredecessor(EphemeralBetree(k, s).value.bcv.view, iset{step.ref});
+      assert IMapRemove1(EphemeralBetree(k, s).value.bcv.view, step.ref)
+          == IMapRemove(EphemeralBetree(k, s).value.bcv.view, iset{step.ref});
+      assert BI.GC(Ik(k).bck, EphemeralBetree(k, s).value.bcv, EphemeralBetree(k, s').value.bcv, iset{step.ref});
+      assert BT.GC(Ik(k), EphemeralBetree(k, s).value, EphemeralBetree(k, s').value, UI.NoOp, iset{step.ref});
+      BT.GCStepRefines(Ik(k), EphemeralBetree(k, s).value, EphemeralBetree(k, s').value, UI.NoOp, iset{step.ref});
+    }
+
+    if vop.FreezeOp? {
+    }
+    else if vop.CrashOp? {
+    }
+    else if vop.SendPersistentLocOp? {
+    }
+    else if vop.SendFrozenLocOp? {
+    }
+    else if vop.CleanUpOp? {
+    }
+    else if Ref.IsTransactionStep(BCS.MachineStep(dop, step)) {
+    }
+    else if vop.StatesInternalOp? {
+      if Ref.UpdateAllEq(k, s, s') {
+      }
+      else if Ref.UpdateDiskChange(k, s, s') {
+      }
+      else if Ref.UpdateUnalloc(k, s, s', BCS.MachineStep(dop, step)) {
+      }
+      else {
+      }
+    }
+    else if vop.JournalInternalOp? {
+      assert Ref.UpdateAllEq(k, s, s');
+    }
+    else if vop.PushSyncOp? {
+      assert Ref.UpdateAllEq(k, s, s');
+    }
+    else if vop.PopSyncOp? {
+      assert Ref.UpdateAllEq(k, s, s');
+    }
+    else if vop.AdvanceOp? {
+    }
+    else {
+      assert false;
+    }
+  }
+
+  lemma CrashStepPreservesInv(k: Constants, s: Variables, s': Variables, vop: VOp)
+    requires Inv(k, s)
+    requires Crash(k, s, s', vop)
+    ensures Inv(k, s')
+  {
+    Ref.StepGraphs(k, s, s', vop, BCS.CrashStep);
+  }
+
+  lemma NextStepPreservesInv(k: Constants, s: Variables, s': Variables, vop: VOp, step: Step)
+    requires Inv(k, s)
+    requires NextStep(k, s, s', vop, step)
+    ensures Inv(k, s')
+  {
+    match step {
+      case MachineStep(dop) => {
+        var machineStep :| M.NextStep(k.machine, s.machine, s'.machine, dop, vop, machineStep);
+        match machineStep {
+          case BetreeMoveStep(betreeStep) => BetreeMoveStepPreservesInv(k, s, s', dop, vop, betreeStep);
+          case BlockCacheMoveStep(blockCacheStep) => BlockCacheMoveStepPreservesInv(k, s, s', dop, vop, blockCacheStep);
+        }
+      }
+      case CrashStep => CrashStepPreservesInv(k, s, s', vop);
+    }
+  }
+
+  lemma NextPreservesInv(k: Constants, s: Variables, s': Variables, vop: VOp)
+  requires Inv(k, s)
+  requires Next(k, s, s', vop)
+  ensures Inv(k, s')
+  {
+    var step :| NextStep(k, s, s', vop, step);
+    NextStepPreservesInv(k, s, s', vop, step);
+  }
+}
