BlockCacheSystem/BetreeSystem_Refines_StatesViewPivotBetree.i.dfy
@@ -1,0 +1,195 @@
+include "../PivotBetree/PivotBetree_Refines_Betree.i.dfy"
+include "../BlockCacheSystem/BlockCache.i.dfy"
+include "../lib/Base/Maps.s.dfy"
+include "../lib/Base/sequences.i.dfy"
+include "BetreeSystem.i.dfy"
+include "../PivotBetree/StatesViewPivotBetree.i.dfy"
+//
+// Take the whole crash-safe BlockCacheSystem, and constrain it to
+// run the (Pivot)Betree as its client, thereby yielding a 3-state-crash-safe
+// Betree. (We'll eventually tie that up the stack to get a 3-state-crash-safe
+// map.)
+//
+
+module BetreeSystem_Refines_StatesViewPivotBetree {
+  import opened Maps
+  import opened Sequences
+
+  import System = BetreeSystem
+  import View = StatesViewPivotBetree
+
+  import opened PivotBetreeSpec`Spec
+  import opened ViewOp
+  import opened DiskLayout
+  import BC = BlockCache
+  import BCS = BlockSystem
+  import BT = PivotBetree
+  import BI = PivotBetreeBlockInterface
+  import Ref = BlockSystem_Refines_StatesView
+  import D = BlockDisk
+
+  import M = BetreeCache
+
+  function Ik(k: System.Constants) : View.Constants
+  {
+    View.Constants(BT.Constants(BI.Constants()))
+  }
+
+  function I(k: System.Constants, s: System.Variables) : View.Variables
+  requires System.Inv(k, s)
+  {
+    View.Variables(
+      System.BetreeDisk(k, s),
+      BCS.PersistentLoc(k, s),
+      BCS.FrozenLoc(k, s),
+      System.FrozenBetree(k, s),
+      System.EphemeralBetree(k, s)
+    )
+  }
+
+  // Proofs
+
+  lemma RefinesInit(k: System.Constants, s: System.Variables, loc: Location)
+    requires System.Init(k, s, loc)
+    ensures System.Inv(k, s)
+    ensures View.Init(Ik(k), I(k, s), loc)
+  {
+    BCS.InitImpliesInv(k, s, loc);
+    BT.InitImpliesInv(Ik(k).k, System.BetreeDisk(k, s)[loc]);
+    BCS.InitGraphs(k, s, loc);
+  }
+
+  lemma BetreeMoveStepRefines(k: System.Constants, s: System.Variables, s': System.Variables, dop: D.DiskOp, vop: VOp, betreeStep: BetreeStep)
+    requires System.Inv(k, s)
+    requires M.BetreeMove(k.machine, s.machine, s'.machine, dop, vop, betreeStep)
+    requires D.Next(k.disk, s.disk, s'.disk, dop)
+    ensures System.Inv(k, s')
+    ensures View.Next(Ik(k), I(k, s), I(k, s'), vop)
+  {
+    var transactionStep := BC.TransactionStep(BetreeStepOps(betreeStep));
+    Ref.StepGraphs(k, s, s', vop, BCS.MachineStep(dop, transactionStep));
+    Ref.RefinesReads(k, s, BetreeStepReads(betreeStep));
+    assert BT.NextStep(Ik(k).k, System.EphemeralBetree(k, s).value, System.EphemeralBetree(k, s').value, vop.uiop, BT.BetreeStep(betreeStep));
+    BT.NextPreservesInv(Ik(k).k, System.EphemeralBetree(k, s).value, System.EphemeralBetree(k, s').value, vop.uiop);
+    assert View.NextStep(Ik(k), I(k, s), I(k, s'), vop, View.AdvanceStep);
+  }
+
+  lemma BlockCacheMoveStepRefines(k: System.Constants, s: System.Variables, s': System.Variables, dop: D.DiskOp, vop: VOp, step: BC.Step)
+    requires System.Inv(k, s)
+    requires !step.TransactionStep?
+    requires M.BlockCacheMove(k.machine, s.machine, s'.machine, dop, vop, step)
+    requires D.Next(k.disk, s.disk, s'.disk, dop)
+    requires (vop.SendPersistentLocOp? ==>
+      BCS.Inv(k, s) ==>
+        && vop.loc in Ref.DiskGraphMap(k, s)
+        && BT.Inv(Ik(k).k, BT.Variables(BI.Variables(Ref.DiskGraphMap(k, s)[vop.loc])))
+    )
+
+    ensures System.Inv(k, s')
+    ensures View.Next(Ik(k), I(k, s), I(k, s'), vop)
+  {
+    Ref.StepGraphs(k, s, s', vop, BCS.MachineStep(dop, step));
+    if (step.UnallocStep?) {
+      //assert BI.GC(Ik(k).bck, EphemeralBetree(k, s).bcv, s'.bcv, refs)
+      Ref.UnallocStepMeetsGCConditions(k, s, s', dop, vop, step.ref);
+      /*assert step.ref in EphemeralBetree(k, s).bcv.view;
+      assert iset{step.ref} !! BI.LiveReferences(Ik(k).bck, EphemeralBetree(k, s).bcv);
+      assert BI.ClosedUnderPredecessor(EphemeralBetree(k, s).bcv.view, iset{step.ref});
+      assert IMapRemove1(EphemeralBetree(k, s).bcv.view, step.ref)
+          == IMapRemove(EphemeralBetree(k, s).bcv.view, iset{step.ref});*/
+      assert BT.GC(Ik(k).k, System.EphemeralBetree(k, s).value, System.EphemeralBetree(k, s').value, UI.NoOp, iset{step.ref});
+      BT.GCStepRefines(Ik(k).k, System.EphemeralBetree(k, s).value, System.EphemeralBetree(k, s').value, UI.NoOp, iset{step.ref});
+
+      assert BT.NextStep(Ik(k).k, I(k, s).ephemeralState.value, I(k, s').ephemeralState.value, UI.NoOp, BT.GCStep(iset{step.ref}));
+
+      assert View.Advance(Ik(k), I(k, s), I(k, s'), vop);
+      assert View.NextStep(Ik(k), I(k, s), I(k, s'), vop, View.AdvanceStep);
+    } else {
+      if vop.FreezeOp? {
+        assert View.NextStep(Ik(k), I(k, s), I(k, s'), vop, View.FreezeStep);
+      }
+      else if vop.CrashOp? {
+        assert View.NextStep(Ik(k), I(k, s), I(k, s'), vop, View.CrashStep);
+      }
+      else if vop.SendPersistentLocOp? {
+        assert View.ObtainPersistentLoc(Ik(k), I(k, s), I(k, s'), vop);
+        assert View.NextStep(Ik(k), I(k, s), I(k, s'), vop, View.ObtainPersistentLocStep);
+      }
+      else if vop.SendFrozenLocOp? {
+        assert View.NextStep(Ik(k), I(k, s), I(k, s'), vop, View.ProvideFrozenLocStep);
+      }
+      else if vop.CleanUpOp? {
+        assert View.NextStep(Ik(k), I(k, s), I(k, s'), vop, View.ForgetOldStep);
+      }
+      else if vop.AdvanceOp? {
+        assert false;
+      }
+      else if vop.StatesInternalOp? {
+        if Ref.UpdateAllEq(k, s, s') {
+          assert View.NextStep(Ik(k), I(k, s), I(k, s'), vop, View.StutterStep);
+        }
+        else if Ref.UpdateDiskChange(k, s, s') {
+          assert View.NextStep(Ik(k), I(k, s), I(k, s'), vop, View.DiskChangeStep);
+        }
+        else if Ref.UpdateUnalloc(k, s, s', BCS.MachineStep(dop, step)) {
+          assert false;
+        }
+        else {
+        }
+      }
+      else if vop.JournalInternalOp? {
+        assert Ref.UpdateAllEq(k, s, s');
+        assert View.NextStep(Ik(k), I(k, s), I(k, s'), vop, View.StutterStep);
+      }
+      else if vop.PushSyncOp? {
+        assert Ref.UpdateAllEq(k, s, s');
+        assert View.NextStep(Ik(k), I(k, s), I(k, s'), vop, View.StutterStep);
+      }
+      else if vop.PopSyncOp? {
+        assert Ref.UpdateAllEq(k, s, s');
+        assert View.NextStep(Ik(k), I(k, s), I(k, s'), vop, View.StutterStep);
+      }
+      else {
+        assert false;
+      }
+    }
+  }
+
+  lemma CrashStepRefines(k: System.Constants, s: System.Variables, s': System.Variables, vop: VOp)
+    requires System.Inv(k, s)
+    requires System.Crash(k, s, s', vop)
+    ensures System.Inv(k, s')
+    ensures View.Next(Ik(k), I(k, s), I(k, s'), vop)
+  {
+    Ref.StepGraphs(k, s, s', vop, BCS.CrashStep);
+    assert View.NextStep(Ik(k), I(k, s), I(k, s'), vop, View.CrashStep);
+  }
+
+  lemma NextStepRefines(k: System.Constants, s: System.Variables, s': System.Variables, vop: VOp, step: System.Step)
+    requires System.Inv(k, s)
+    requires System.NextStep(k, s, s', vop, step)
+    ensures System.Inv(k, s')
+    ensures View.Next(Ik(k), I(k, s), I(k, s'), vop)
+  {
+    match step {
+      case MachineStep(dop) => {
+        var machineStep :| M.NextStep(k.machine, s.machine, s'.machine, dop, vop, machineStep);
+        match machineStep {
+          case BetreeMoveStep(betreeStep) => BetreeMoveStepRefines(k, s, s', dop, vop, betreeStep);
+          case BlockCacheMoveStep(blockCacheStep) => BlockCacheMoveStepRefines(k, s, s', dop, vop, blockCacheStep);
+        }
+      }
+      case CrashStep => CrashStepRefines(k, s, s', vop);
+    }
+  }
+
+  lemma RefinesNext(k: System.Constants, s: System.Variables, s': System.Variables, vop: VOp)
+    requires System.Inv(k, s)
+    requires System.Next(k, s, s', vop)
+    ensures System.Inv(k, s')
+    ensures View.Next(Ik(k), I(k, s), I(k, s'), vop);
+  {
+    var step :| System.NextStep(k, s, s', vop, step);
+    NextStepRefines(k, s, s', vop, step);
+  }
+}
