BlockCacheSystem/BlockSystem_Refines_StatesView.i.dfy
@@ -1,0 +1,426 @@
+include "../BlockCacheSystem/BlockSystem.i.dfy"
+include "../Versions/StatesView.i.dfy"
+include "../lib/Base/Maps.s.dfy"
+include "../lib/Base/sequences.i.dfy"
+
+module BlockSystem_Refines_StatesView {
+  import opened G = PivotBetreeGraph
+  import System = BlockSystem
+  import opened AsyncSectorDiskModelTypes
+
+  import opened Maps
+  import opened Sequences
+  import opened Options
+  import opened NativeTypes
+  import opened ViewOp
+  import opened DiskLayout
+
+  import BC = BlockCache
+  import BI = PivotBetreeBlockInterface
+  import D = BlockDisk
+  type DiskOp = BC.DiskOp
+
+  function Ik(k: System.Constants) : BI.Constants
+  {
+    BI.Constants()
+  }
+
+  predicate IsTransactionStep(step: System.Step)
+  {
+    && step.MachineStep?
+    && step.machineStep.TransactionStep?
+  }
+
+  function DiskGraphMap(k: System.Constants, s: System.Variables)
+    : imap<Location, imap<Reference, Node>>
+  {
+    System.DiskGraphMap(k, s)
+  }
+
+  function FrozenGraph(k: System.Constants, s: System.Variables) : Option<imap<Reference, Node>>
+  {
+    System.FrozenGraphOpt(k, s)
+  }
+
+  function EphemeralGraph(k: System.Constants, s: System.Variables) : Option<imap<Reference, Node>>
+  {
+    System.EphemeralGraphOpt(k, s)
+  }
+
+  function PersistentLoc(k: System.Constants, s: System.Variables) : Option<Location>
+  {
+    System.PersistentLoc(k, s)
+  }
+
+  function FrozenLoc(k: System.Constants, s: System.Variables) : Option<Location>
+  {
+    System.FrozenLoc(k, s)
+  }
+
+  predicate UpdateAllEq(
+    k: System.Constants,
+    s: System.Variables,
+    s': System.Variables)
+  {
+    && System.Inv(k, s)
+    && System.Inv(k, s')
+    && DiskGraphMap(k, s') == DiskGraphMap(k, s)
+    && FrozenGraph(k, s') == FrozenGraph(k, s)
+    && EphemeralGraph(k, s') == EphemeralGraph(k, s)
+    && PersistentLoc(k, s') == PersistentLoc(k, s)
+    && FrozenLoc(k, s') == FrozenLoc(k, s)
+  }
+
+  predicate UpdateCrash(
+    k: System.Constants,
+    s: System.Variables,
+    s': System.Variables)
+  {
+    && System.Inv(k, s)
+    && System.Inv(k, s')
+    && System.DiskChangesPreservesPersistentAndFrozen(k, s, s')
+    && FrozenGraph(k, s') == None
+    && EphemeralGraph(k, s') == None
+    && PersistentLoc(k, s') == None
+    && FrozenLoc(k, s') == None
+  }
+
+  predicate UpdateObtainPersistentLoc(
+    k: System.Constants,
+    s: System.Variables,
+    s': System.Variables,
+    vop: VOp)
+  {
+    && vop.SendPersistentLocOp?
+    && System.Inv(k, s)
+    && System.Inv(k, s')
+    && PersistentLoc(k, s) == None
+    && DiskGraphMap(k, s') == DiskGraphMap(k, s)
+    && FrozenGraph(k, s') == FrozenGraph(k, s)
+    && vop.loc in DiskGraphMap(k, s)
+    && EphemeralGraph(k, s') == Some(DiskGraphMap(k, s)[vop.loc])
+    && PersistentLoc(k, s') == Some(vop.loc)
+    && FrozenLoc(k, s') == FrozenLoc(k, s)
+  }
+
+  predicate UpdateFreeze(
+    k: System.Constants,
+    s: System.Variables,
+    s': System.Variables)
+  {
+    && System.Inv(k, s)
+    && System.Inv(k, s')
+    && DiskGraphMap(k, s') == DiskGraphMap(k, s)
+    && FrozenGraph(k, s') == EphemeralGraph(k, s)
+    && EphemeralGraph(k, s') == EphemeralGraph(k, s)
+    && PersistentLoc(k, s') == PersistentLoc(k, s)
+    && FrozenLoc(k, s') == None
+  }
+
+  predicate UpdateDiskChange(
+    k: System.Constants,
+    s: System.Variables,
+    s': System.Variables)
+  {
+    && System.Inv(k, s)
+    && System.Inv(k, s')
+    && System.DiskChangesPreservesPersistentAndFrozen(k, s, s')
+    && FrozenGraph(k, s') == FrozenGraph(k, s)
+    && EphemeralGraph(k, s') == EphemeralGraph(k, s)
+    && PersistentLoc(k, s') == PersistentLoc(k, s)
+    && FrozenLoc(k, s') == FrozenLoc(k, s)
+  }
+
+  predicate UpdateProvideFrozenLoc(
+    k: System.Constants,
+    s: System.Variables,
+    s': System.Variables,
+    vop: VOp)
+  {
+    && vop.SendFrozenLocOp?
+    && FrozenLoc(k, s) == None
+    && FrozenLoc(k, s') == Some(vop.loc)
+    && FrozenGraph(k, s).Some?
+    && FrozenLoc(k, s').value in DiskGraphMap(k, s)
+    && DiskGraphMap(k, s)[FrozenLoc(k, s').value] == FrozenGraph(k, s).value
+    && DiskGraphMap(k, s') == DiskGraphMap(k, s)
+    && FrozenGraph(k, s') == FrozenGraph(k, s)
+    && EphemeralGraph(k, s') == EphemeralGraph(k, s)
+    && PersistentLoc(k, s') == PersistentLoc(k, s)
+  }
+
+  predicate UpdateForgetOld(
+    k: System.Constants,
+    s: System.Variables,
+    s': System.Variables)
+  {
+    && DiskGraphMap(k, s') == DiskGraphMap(k, s)
+    && FrozenGraph(k, s') == None
+    && EphemeralGraph(k, s') == EphemeralGraph(k, s)
+    && FrozenLoc(k, s') == None
+    && PersistentLoc(k, s') == FrozenLoc(k, s)
+  }
+
+  predicate UpdateUnalloc(
+    k: System.Constants,
+    s: System.Variables,
+    s': System.Variables,
+    step: System.Step)
+  {
+    && System.Inv(k, s)
+    && System.Inv(k, s')
+
+    && step.MachineStep?
+    && step.machineStep.UnallocStep?
+
+    && DiskGraphMap(k, s') == DiskGraphMap(k, s)
+    && PersistentLoc(k, s') == PersistentLoc(k, s)
+    && FrozenLoc(k, s') == FrozenLoc(k, s)
+    && FrozenGraph(k, s') == FrozenGraph(k, s)
+
+    && EphemeralGraph(k, s).Some?
+    && EphemeralGraph(k, s').Some?
+
+    && EphemeralGraph(k, s').value == IMapRemove1(EphemeralGraph(k, s).value, step.machineStep.ref)
+  }
+
+  predicate UpdateTransaction(
+    k: System.Constants,
+    s: System.Variables,
+    s': System.Variables,
+    step: System.Step)
+  {
+    && IsTransactionStep(step)
+    && System.Inv(k, s)
+    && System.Inv(k, s')
+
+    && step.MachineStep?
+    && step.machineStep.TransactionStep?
+
+    && DiskGraphMap(k, s') == DiskGraphMap(k, s)
+    && PersistentLoc(k, s') == PersistentLoc(k, s)
+    && FrozenLoc(k, s') == FrozenLoc(k, s)
+    && FrozenGraph(k, s') == FrozenGraph(k, s)
+
+    && EphemeralGraph(k, s).Some?
+    && EphemeralGraph(k, s').Some?
+
+    && BI.OpTransaction(BI.Constants(),
+            BI.Variables(EphemeralGraph(k, s).value),
+            BI.Variables(EphemeralGraph(k, s').value),
+            step.machineStep.ops)
+  }
+
+  lemma OpTransactionUpdate(k: System.Constants, s: System.Variables, s': System.Variables, ops: seq<Op>)
+  requires System.Inv(k, s)
+  requires s.disk == s'.disk
+  requires BC.OpTransaction(k.machine, s.machine, s'.machine, ops)
+  requires s.machine.Ready?
+  ensures System.Inv(k, s')
+  ensures DiskGraphMap(k, s') == DiskGraphMap(k, s)
+  ensures PersistentLoc(k, s') == PersistentLoc(k, s)
+  ensures FrozenLoc(k, s') == FrozenLoc(k, s)
+  ensures FrozenGraph(k, s') == FrozenGraph(k, s)
+  ensures s'.machine.Ready?
+  ensures EphemeralGraph(k, s).Some?
+  ensures EphemeralGraph(k, s').Some?
+  ensures BI.OpTransaction(BI.Constants(),
+            BI.Variables(EphemeralGraph(k, s).value),
+            BI.Variables(EphemeralGraph(k, s').value),
+            ops)
+
+  decreases |ops|
+  {
+    //reveal_PersistentGraph();
+    //reveal_FrozenGraph();
+    //reveal_EphemeralGraph();
+    if |ops| == 0 {
+    } else if |ops| == 1 {
+      System.OpPreservesInv(k, s, s', ops[0]);
+      match ops[0] {
+        case WriteOp(ref, block) => {
+          System.DirtyStepUpdatesGraph(k, s, s', ref, block);
+          assert BI.Write(BI.Constants(),
+              BI.Variables(EphemeralGraph(k, s).value),
+              BI.Variables(EphemeralGraph(k, s').value),
+              ref, block);
+          assert BI.OpStep(BI.Constants(),
+              BI.Variables(EphemeralGraph(k, s).value),
+              BI.Variables(EphemeralGraph(k, s').value),
+              ops[0]);
+        }
+        case AllocOp(ref, block) => {
+          System.AllocStepUpdatesGraph(k, s, s', ref, block);
+          assert BI.OpStep(BI.Constants(),
+              BI.Variables(EphemeralGraph(k, s).value),
+              BI.Variables(EphemeralGraph(k, s').value),
+              ops[0]);
+        }
+      }
+    } else {
+      var ops1, mid, ops2 := BC.SplitTransaction(k.machine, s.machine, s'.machine, ops);
+      var smid := AsyncSectorDiskModelVariables(mid, s.disk);
+      OpTransactionUpdate(k, s, smid, ops1);
+      OpTransactionUpdate(k, smid, s', ops2);
+      BI.JoinTransactions(BI.Constants(),
+        BI.Variables(EphemeralGraph(k, s).value),
+        BI.Variables(EphemeralGraph(k, smid).value),
+        BI.Variables(EphemeralGraph(k, s').value),
+        ops1, ops2);
+    }
+  }
+
+  lemma TransactionUpdate(k: System.Constants, s: System.Variables, s': System.Variables, vop: VOp, step: System.Step)
+  requires System.Inv(k, s)
+  requires s.disk == s'.disk
+  requires step.MachineStep?
+  requires step.machineStep.TransactionStep?
+  requires BC.Transaction(k.machine, s.machine, s'.machine, D.NoDiskOp, vop, step.machineStep.ops)
+
+  ensures System.Inv(k, s')
+  ensures UpdateTransaction(k, s, s', step)
+  {
+    OpTransactionUpdate(k, s, s', step.machineStep.ops);
+  }
+
+  lemma RefinesReads(k: System.Constants, s: System.Variables, ops: seq<ReadOp>)
+  requires System.Inv(k, s)
+  requires BC.Reads(k.machine, s.machine, ops)
+  requires s.machine.Ready?
+  ensures EphemeralGraph(k, s).Some?
+  ensures BI.Reads(BI.Constants(), BI.Variables(EphemeralGraph(k, s).value), ops)
+  {
+    //reveal_EphemeralGraph();
+    forall op | op in ops
+    ensures BI.ReadStep(BI.Constants, BI.Variables(EphemeralGraph(k, s).value), op)
+    {
+      System.EphemeralGraphRead(k, s, op);
+      //assert s.machine.cache[op.ref] == op.node;
+      //assert op.ref in EphemeralGraph(k, s);
+      //assert EphemeralGraph(k, s)[op.ref] == op.node;
+    }
+  }
+
+  lemma UnallocStepMeetsGCConditions(k: System.Constants, s: System.Variables, s': System.Variables,
+      dop: DiskOp, vop: VOp, ref: Reference)
+  requires System.Inv(k, s)
+  requires s'.disk == s.disk
+  requires BC.Unalloc(k.machine, s.machine, s'.machine, dop, vop, ref)
+  ensures EphemeralGraph(k, s).Some?
+  ensures EphemeralGraph(k, s').Some?
+  ensures BI.CanGCRefs(BI.Constants(), BI.Variables(EphemeralGraph(k, s).value), iset{ref})
+  ensures System.Inv(k, s')
+  ensures ref in EphemeralGraph(k, s).value
+  ensures EphemeralGraph(k, s').value == IMapRemove1(EphemeralGraph(k, s).value, ref)
+  {
+    System.UnallocStepPreservesInv(k, s, s', dop, vop, ref);
+    System.UnallocStepUpdatesGraph(k, s, s', dop, vop, ref);
+    //reveal_EphemeralGraph();
+    if (ref in BI.LiveReferences(BI.Constants(), BI.Variables(EphemeralGraph(k, s).value))) {
+      assert BI.ReachableReference(BI.Constants(), BI.Variables(EphemeralGraph(k, s).value), ref);
+      var lookup :| BI.LookupIsValid(BI.Constants(), BI.Variables(EphemeralGraph(k, s).value), lookup) && Last(lookup) == ref;
+      assert |lookup| > 1;
+      var pred := lookup[|lookup| - 2];
+      assert ref in G.Successors(EphemeralGraph(k, s).value[pred]);
+      assert false;
+    }
+  }
+
+  // This is the uber lemma that explains how the graphs transform
+  // for all the different step types
+
+  lemma StepGraphs(k: System.Constants, s: System.Variables, s': System.Variables, vop: VOp, step: System.Step)
+  requires System.Inv(k, s)
+  requires System.NextStep(k, s, s', vop, step)
+  ensures System.Inv(k, s')
+
+  ensures vop.FreezeOp? ==>
+      || UpdateFreeze(k, s, s')
+
+  ensures vop.CrashOp? ==>
+      UpdateCrash(k, s, s')
+
+  ensures vop.SendPersistentLocOp? ==>
+      UpdateObtainPersistentLoc(k, s, s', vop)
+
+  ensures vop.SendFrozenLocOp? ==>
+      UpdateProvideFrozenLoc(k, s, s', vop)
+
+  ensures vop.CleanUpOp? ==>
+      UpdateForgetOld(k, s, s')
+
+  ensures vop.AdvanceOp? ==>
+      || UpdateTransaction(k, s, s', step)
+      || UpdateUnalloc(k, s, s', step)
+
+  ensures vop.StatesInternalOp? ==> (
+      || UpdateAllEq(k, s, s')
+      || UpdateDiskChange(k, s, s')
+    )
+
+  ensures vop.JournalInternalOp? ==>
+      UpdateAllEq(k, s, s')
+  ensures vop.PushSyncOp? ==>
+      UpdateAllEq(k, s, s')
+  ensures vop.PopSyncOp? ==>
+      UpdateAllEq(k, s, s')
+  {
+    System.NextStepPreservesInv(k, s, s', vop, step);
+
+    match step {
+      case MachineStep(dop, machineStep) => {
+        match machineStep {
+          case WriteBackNodeReqStep(ref) => {
+            System.WriteBackNodeReqStepPreservesGraphs(k, s, s', dop, vop, ref);
+          }
+          case WriteBackNodeRespStep => {
+            System.WriteBackNodeRespStepPreservesGraphs(k, s, s', dop, vop);
+          }
+          case WriteBackIndirectionTableReqStep => {
+            System.WriteBackIndirectionTableReqStepPreservesGraphs(k, s, s', dop, vop);
+          }
+          case WriteBackIndirectionTableRespStep => {
+            System.WriteBackIndirectionTableRespStepPreservesGraphs(k, s, s', dop, vop);
+          }
+          case UnallocStep(ref: Reference) => {
+            System.UnallocStepUpdatesGraph(k, s, s', dop, vop, ref);
+            assert UpdateUnalloc(k, s, s', step);
+          }
+          case PageInNodeReqStep(ref: Reference) => {
+            System.PageInNodeReqStepPreservesGraphs(k, s, s', dop, vop, ref);
+          }
+          case PageInNodeRespStep => {
+            System.PageInNodeRespStepPreservesGraphs(k, s, s', dop, vop);
+          }
+          case PageInIndirectionTableReqStep => {
+            System.PageInIndirectionTableReqStepPreservesGraphs(k, s, s', dop, vop);
+          }
+          case PageInIndirectionTableRespStep => {
+            System.PageInIndirectionTableRespStepPreservesGraphs(k, s, s', dop, vop);
+          }
+          case EvictStep(ref: Reference) => {
+            System.EvictStepPreservesGraphs(k, s, s', dop, vop, ref);
+          }
+          case FreezeStep => {
+            System.FreezeStepPreservesGraphs(k, s, s', dop, vop);
+          }
+          case CleanUpStep => {
+            System.CleanUpStepPreservesGraphs(k, s, s', dop, vop);
+          }
+          case ReceiveLocStep => {
+            System.ReceiveLocStepPreservesGraphs(k, s, s', dop, vop);
+            assert UpdateObtainPersistentLoc(k, s, s', vop);
+          }
+          case NoOpStep => {
+            System.NoOpStepPreservesGraphs(k, s, s', dop, vop);
+          }
+          case TransactionStep(ops) => TransactionUpdate(k, s, s', vop, step);
+        }
+      }
+      case CrashStep => {
+        System.CrashPreservesGraphs(k, s, s', vop);
+        assert UpdateCrash(k, s, s');
+      }
+    }
+  }
+}
