Impl/CommitterCommitModel.i.dfy
@@ -1,0 +1,836 @@
+include "CommitterModel.i.dfy"
+include "StateModel.i.dfy"
+include "IOModel.i.dfy"
+
+module CommitterCommitModel {
+  import opened NativeTypes
+  import opened Options
+
+  import opened DiskLayout
+  import opened InterpretationDiskOps
+  import opened ViewOp
+  import JC = JournalCache
+  import opened Journal
+  import opened JournalBytes
+  import opened DiskOpModel
+  import SectorType
+
+  import opened CommitterModel
+  import opened StateModel
+  import opened IOModel
+
+  function SyncReqs2to1Iterate(
+      m: MutableMapModel.LinearHashMap<JC.SyncReqStatus>,
+      it: MutableMapModel.Iterator<JC.SyncReqStatus>,
+      m0: MutableMapModel.LinearHashMap<JC.SyncReqStatus>)
+    : (m' : MutableMapModel.LinearHashMap<JC.SyncReqStatus>)
+  requires MutableMapModel.Inv(m)
+  requires MutableMapModel.WFIter(m, it)
+  requires MutableMapModel.Inv(m0)
+  requires m0.contents.Keys == it.s
+  ensures MutableMapModel.Inv(m')
+  decreases it.decreaser
+  {
+    if it.next.Done? then
+      m0
+    else (
+      MutableMapModel.LemmaIterIndexLtCount(m, it);
+      MutableMapModel.CountBound(m);
+      SyncReqs2to1Iterate(
+        m,
+        MutableMapModel.IterInc(m, it),
+        MutableMapModel.Insert(m0, it.next.key,
+            (if it.next.value == JC.State2 then JC.State1 else it.next.value))
+      )
+    )
+  }
+
+  function {:opaque} SyncReqs2to1(m: MutableMapModel.LinearHashMap<JC.SyncReqStatus>)
+      : (m' : MutableMapModel.LinearHashMap<JC.SyncReqStatus>)
+  requires MutableMapModel.Inv(m)
+  ensures MutableMapModel.Inv(m')
+  {
+    SyncReqs2to1Iterate(m,
+      MutableMapModel.IterStart(m),
+      MutableMapModel.Constructor(128))
+  }
+
+  lemma SyncReqs2to1Correct(m: MutableMapModel.LinearHashMap<JC.SyncReqStatus>)
+  requires MutableMapModel.Inv(m)
+  ensures SyncReqs2to1(m).contents == JC.syncReqs2to1(m.contents)
+  {
+    reveal_SyncReqs2to1();
+    var it := MutableMapModel.IterStart(m);
+    var m0 := MutableMapModel.Constructor(128);
+    while !it.next.Done?
+    invariant MutableMapModel.Inv(m)
+    invariant MutableMapModel.WFIter(m, it)
+    invariant MutableMapModel.Inv(m0)
+    invariant m0.contents.Keys == it.s
+    invariant forall id | id in it.s ::
+        m0.contents[id] == (if m.contents[id] == JC.State2 then JC.State1 else m.contents[id])
+    invariant SyncReqs2to1(m) == SyncReqs2to1Iterate(m, it, m0)
+    decreases it.decreaser
+    {
+      MutableMapModel.LemmaIterIndexLtCount(m, it);
+      MutableMapModel.CountBound(m);
+      m0 := MutableMapModel.Insert(m0, it.next.key,
+          (if it.next.value == JC.State2 then JC.State1 else it.next.value));
+      it := MutableMapModel.IterInc(m, it);
+    }
+  }
+
+  function SyncReqs3to2Iterate(
+      m: MutableMapModel.LinearHashMap<JC.SyncReqStatus>,
+      it: MutableMapModel.Iterator<JC.SyncReqStatus>,
+      m0: MutableMapModel.LinearHashMap<JC.SyncReqStatus>)
+    : (m' : MutableMapModel.LinearHashMap<JC.SyncReqStatus>)
+  requires MutableMapModel.Inv(m)
+  requires MutableMapModel.WFIter(m, it)
+  requires MutableMapModel.Inv(m0)
+  requires m0.contents.Keys == it.s
+  ensures MutableMapModel.Inv(m')
+  decreases it.decreaser
+  {
+    if it.next.Done? then
+      m0
+    else (
+      MutableMapModel.LemmaIterIndexLtCount(m, it);
+      MutableMapModel.CountBound(m);
+      SyncReqs3to2Iterate(
+        m,
+        MutableMapModel.IterInc(m, it),
+        MutableMapModel.Insert(m0, it.next.key,
+            (if it.next.value == JC.State3 then JC.State2 else it.next.value))
+      )
+    )
+  }
+
+  function {:opaque} SyncReqs3to2(m: MutableMapModel.LinearHashMap<JC.SyncReqStatus>)
+      : (m' : MutableMapModel.LinearHashMap<JC.SyncReqStatus>)
+  requires MutableMapModel.Inv(m)
+  ensures MutableMapModel.Inv(m')
+  {
+    SyncReqs3to2Iterate(m,
+      MutableMapModel.IterStart(m),
+      MutableMapModel.Constructor(128))
+  }
+
+  lemma SyncReqs3to2Correct(m: MutableMapModel.LinearHashMap<JC.SyncReqStatus>)
+  requires MutableMapModel.Inv(m)
+  ensures SyncReqs3to2(m).contents == JC.syncReqs3to2(m.contents)
+  {
+    reveal_SyncReqs3to2();
+    var it := MutableMapModel.IterStart(m);
+    var m0 := MutableMapModel.Constructor(128);
+    while !it.next.Done?
+    invariant MutableMapModel.Inv(m)
+    invariant MutableMapModel.WFIter(m, it)
+    invariant MutableMapModel.Inv(m0)
+    invariant m0.contents.Keys == it.s
+    invariant forall id | id in it.s ::
+        m0.contents[id] == (if m.contents[id] == JC.State3 then JC.State2 else m.contents[id])
+    invariant SyncReqs3to2(m) == SyncReqs3to2Iterate(m, it, m0)
+    decreases it.decreaser
+    {
+      MutableMapModel.LemmaIterIndexLtCount(m, it);
+      MutableMapModel.CountBound(m);
+      m0 := MutableMapModel.Insert(m0, it.next.key,
+          (if it.next.value == JC.State3 then JC.State2 else it.next.value));
+      it := MutableMapModel.IterInc(m, it);
+    }
+  }
+
+  function method start_pos_add(a: uint64, b: uint64) : uint64
+  requires 0 <= a <= NumJournalBlocks()
+  requires 0 <= b <= NumJournalBlocks()
+  {
+    if a + b >= NumJournalBlocks()
+      then a + b - NumJournalBlocks()
+      else a + b
+  }
+
+  function {:opaque} WriteOutJournal(k: Constants, cm: CM, io: IO)
+      : (res : (CM, IO))
+  requires io.IOInit?
+  requires CommitterModel.WF(cm)
+  requires JournalistModel.I(cm.journalist).inMemoryJournalFrozen != []
+        || JournalistModel.I(cm.journalist).inMemoryJournal != []
+  {
+    var writtenJournalLen :=
+        JournalistModel.getWrittenJournalLen(cm.journalist);
+
+    var doingFrozen :=
+      JournalistModel.hasFrozenJournal(cm.journalist);
+
+    var (journalist', j) :=
+      if doingFrozen then
+        JournalistModel.packageFrozenJournal(cm.journalist)
+      else
+        JournalistModel.packageInMemoryJournal(cm.journalist);
+
+    var start := start_pos_add(
+        cm.superblock.journalStart,
+        writtenJournalLen);
+
+    var len := |j| as uint64 / 4096;
+
+    var contiguous := start + len <= NumJournalBlocks();
+
+    var io' := if contiguous then
+      IOReqWrite(io.id, D.ReqWrite(JournalPoint(start), j))
+    else (
+      var cut := (NumJournalBlocks() - start) * 4096;
+      IOReqWrite2(io.id, io.id2,
+          D.ReqWrite(JournalPoint(start), j[..cut]),
+          D.ReqWrite(JournalPoint(0), j[cut..]))
+    );
+
+    var outstandingJournalWrites' := if contiguous
+        then cm.outstandingJournalWrites + {io.id}
+        else cm.outstandingJournalWrites + {io.id, io.id2};
+
+    var frozenJournalPosition' := if doingFrozen
+      then JournalistModel.getWrittenJournalLen(journalist')
+      else cm.frozenJournalPosition;
+
+    var syncReqs' := if doingFrozen
+      then cm.syncReqs
+      else SyncReqs3to2(cm.syncReqs);
+
+    var cm' := cm
+      .(outstandingJournalWrites := outstandingJournalWrites')
+      .(journalist := journalist')
+      .(frozenJournalPosition := frozenJournalPosition')
+      .(syncReqs := syncReqs');
+
+    (cm', io')
+  }
+
+  lemma WriteOutJournalCorrect(k: Constants, cm: CM, io: IO)
+  requires WriteOutJournal.requires(k, cm, io)
+  requires cm.superblockWrite.None?
+  ensures var (cm', io') := WriteOutJournal(k, cm, io);
+    && CommitterModel.WF(cm')
+    && ValidDiskOp(diskOp(io'))
+    && IDiskOp(diskOp(io')).bdop.NoDiskOp?
+    && JC.Next(Ik(k).jc,
+        CommitterModel.I(cm),
+        CommitterModel.I(cm'),
+        IDiskOp(diskOp(io')).jdop,
+        JournalInternalOp)
+  {
+    var (cm', io') := WriteOutJournal(k, cm, io);
+    reveal_WriteOutJournal();
+
+    var writtenJournalLen :=
+        JournalistModel.getWrittenJournalLen(cm.journalist);
+
+    var doingFrozen :=
+      JournalistModel.hasFrozenJournal(cm.journalist);
+
+    var (journalist', j) :=
+      if doingFrozen then
+        JournalistModel.packageFrozenJournal(cm.journalist)
+      else
+        JournalistModel.packageInMemoryJournal(cm.journalist);
+
+    var start := start_pos_add(
+        cm.superblock.journalStart,
+        writtenJournalLen);
+
+    var jr := JournalRangeOfByteSeq(j).value;
+    var len := |j| as uint64 / 4096;
+    var contiguous := start + len <= NumJournalBlocks();
+
+    assert |jr| == len as int;
+
+    if contiguous {
+      assert LocOfReqWrite(diskOp(io').reqWrite)
+          == JournalRangeLocation(start, len);
+      assert ValidDiskOp(diskOp(io'));
+    } else {
+      assert LocOfReqWrite(diskOp(io').reqWrite1)
+          == JournalRangeLocation(start, NumJournalBlocks() - start);
+      assert LocOfReqWrite(diskOp(io').reqWrite2)
+          == JournalRangeLocation(0, len - (NumJournalBlocks() - start));
+      JournalBytesSplit(j, len as int,
+          NumJournalBlocks() as int - start as int);
+      assert ValidDiskOp(diskOp(io'));
+    }
+
+    SyncReqs3to2Correct(cm.syncReqs);
+
+    assert JC.WriteBackJournalReq(Ik(k).jc,
+        CommitterModel.I(cm),
+        CommitterModel.I(cm'),
+        IDiskOp(diskOp(io')).jdop,
+        JournalInternalOp,
+        jr);
+    assert JC.NextStep(Ik(k).jc,
+        CommitterModel.I(cm),
+        CommitterModel.I(cm'),
+        IDiskOp(diskOp(io')).jdop,
+        JournalInternalOp,
+        JC.WriteBackJournalReqStep(jr));
+  }
+
+  predicate writeOutSuperblockAdvanceLog(k: Constants, cm: CM, io: IO,
+      cm': CM, io': IO)
+  requires io.IOInit?
+  requires CommitterModel.WF(cm)
+  {
+    var writtenJournalLen :=
+        JournalistModel.getWrittenJournalLen(cm.journalist);
+    var newSuperblock := SectorType.Superblock(
+      JC.IncrementSuperblockCounter(cm.superblock.counter),
+      cm.superblock.journalStart,
+      writtenJournalLen,
+      cm.superblock.indirectionTableLoc
+    );
+
+    var loc := if cm.whichSuperblock == 0 then Superblock2Location() else Superblock1Location();
+
+    && cm'.superblockWrite.Some?
+    && var id := cm'.superblockWrite.value;
+
+    && RequestWrite(io, loc, SectorSuperblock(newSuperblock),
+        id, io')
+    && cm' == cm
+      .(newSuperblock := Some(newSuperblock))
+      .(superblockWrite := Some(id))
+      .(commitStatus := JC.CommitAdvanceLog)
+  }
+
+  lemma writeOutSuperblockAdvanceLogCorrect(k: Constants, cm: CM, io: IO,
+      cm': CM, io': IO)
+  requires io.IOInit?
+  requires CommitterModel.WF(cm)
+  requires writeOutSuperblockAdvanceLog(k, cm, io, cm', io')
+  requires cm.status == StatusReady
+  requires cm.commitStatus.CommitNone?
+  requires cm.outstandingJournalWrites == {}
+  requires JournalistModel.I(cm.journalist).inMemoryJournalFrozen == []
+  ensures CommitterModel.WF(cm')
+  ensures ValidDiskOp(diskOp(io'))
+  ensures IDiskOp(diskOp(io')).bdop.NoDiskOp?
+  ensures JC.Next(Ik(k).jc,
+        CommitterModel.I(cm),
+        CommitterModel.I(cm'),
+        IDiskOp(diskOp(io')).jdop,
+        JournalInternalOp)
+  {
+    var writtenJournalLen :=
+        JournalistModel.getWrittenJournalLen(cm.journalist);
+    var newSuperblock := SectorType.Superblock(
+      JC.IncrementSuperblockCounter(cm.superblock.counter),
+      cm.superblock.journalStart,
+      writtenJournalLen,
+      cm.superblock.indirectionTableLoc
+    );
+    assert JC.WFSuperblock(newSuperblock);
+
+    var loc := if cm.whichSuperblock == 0 then Superblock2Location() else Superblock1Location();
+
+    var id := cm'.superblockWrite.value;
+
+    RequestWriteCorrect(io, loc, SectorSuperblock(newSuperblock),
+        id, io');
+
+    assert ValidDiskOp(diskOp(io'));
+
+    assert JC.WriteBackSuperblockReq_AdvanceLog(Ik(k).jc,
+        CommitterModel.I(cm),
+        CommitterModel.I(cm'),
+        IDiskOp(diskOp(io')).jdop,
+        JournalInternalOp);
+    assert JC.NextStep(Ik(k).jc,
+        CommitterModel.I(cm),
+        CommitterModel.I(cm'),
+        IDiskOp(diskOp(io')).jdop,
+        JournalInternalOp,
+        JC.WriteBackSuperblockReq_AdvanceLog_Step);
+  }
+
+  predicate {:opaque} writeOutSuperblockAdvanceLocation(k: Constants, cm: CM, io: IO,
+      cm': CM, io': IO)
+  requires io.IOInit?
+  requires CommitterModel.Inv(cm)
+  requires cm.status == StatusReady
+  requires cm.frozenLoc.Some?
+  {
+    var writtenJournalLen :=
+        JournalistModel.getWrittenJournalLen(cm.journalist);
+    var newSuperblock := SectorType.Superblock(
+      JC.IncrementSuperblockCounter(cm.superblock.counter),
+      start_pos_add(
+          cm.superblock.journalStart,
+          cm.frozenJournalPosition),
+      writtenJournalLen - cm.frozenJournalPosition,
+      cm.frozenLoc.value
+    );
+
+    var loc := if cm.whichSuperblock == 0 then Superblock2Location() else Superblock1Location();
+
+    && cm'.superblockWrite.Some?
+    && var id := cm'.superblockWrite.value;
+
+    && RequestWrite(io, loc, SectorSuperblock(newSuperblock),
+        id, io')
+    && cm' == cm
+      .(newSuperblock := Some(newSuperblock))
+      .(superblockWrite := Some(id))
+      .(commitStatus := JC.CommitAdvanceLocation)
+  }
+
+  lemma writeOutSuperblockAdvanceLocationCorrect(k: Constants, cm: CM, io: IO,
+      cm': CM, io': IO)
+  requires io.IOInit?
+  requires CommitterModel.Inv(cm)
+  requires cm.status == StatusReady
+  requires cm.commitStatus.CommitNone?
+  requires cm.outstandingJournalWrites == {}
+  requires cm.frozenLoc.Some?
+  requires writeOutSuperblockAdvanceLocation(k, cm, io, cm', io')
+  requires JournalistModel.I(cm.journalist).inMemoryJournalFrozen == []
+  ensures CommitterModel.WF(cm')
+  ensures ValidDiskOp(diskOp(io'))
+  ensures IDiskOp(diskOp(io')).bdop.NoDiskOp?
+  ensures JC.Next(Ik(k).jc,
+        CommitterModel.I(cm),
+        CommitterModel.I(cm'),
+        IDiskOp(diskOp(io')).jdop,
+        JournalInternalOp)
+  {
+    reveal_writeOutSuperblockAdvanceLocation();
+
+    var writtenJournalLen :=
+        JournalistModel.getWrittenJournalLen(cm.journalist);
+    var newSuperblock := SectorType.Superblock(
+      JC.IncrementSuperblockCounter(cm.superblock.counter),
+      start_pos_add(
+          cm.superblock.journalStart,
+          cm.frozenJournalPosition) as uint64,
+      (writtenJournalLen - cm.frozenJournalPosition) as uint64,
+      cm.frozenLoc.value
+    );
+    assert JC.WFSuperblock(newSuperblock);
+
+    var loc := if cm.whichSuperblock == 0 then Superblock2Location() else Superblock1Location();
+
+    var id := cm'.superblockWrite.value;
+
+    RequestWriteCorrect(io, loc, SectorSuperblock(newSuperblock),
+        id, io');
+
+    assert ValidDiskOp(diskOp(io'));
+
+    assert JC.WriteBackSuperblockReq_AdvanceLocation(Ik(k).jc,
+        CommitterModel.I(cm),
+        CommitterModel.I(cm'),
+        IDiskOp(diskOp(io')).jdop,
+        JournalInternalOp);
+    assert JC.NextStep(Ik(k).jc,
+        CommitterModel.I(cm),
+        CommitterModel.I(cm'),
+        IDiskOp(diskOp(io')).jdop,
+        JournalInternalOp,
+        JC.WriteBackSuperblockReq_AdvanceLocation_Step);
+  }
+
+  function {:opaque} freeze(k: Constants, cm: CM) : (cm': CM)
+  requires CommitterModel.WF(cm)
+  {
+    var writtenJournalLen :=
+        JournalistModel.getWrittenJournalLen(cm.journalist);
+    cm.(frozenLoc := None)
+      .(journalist := JournalistModel.freeze(cm.journalist))
+      .(frozenJournalPosition := writtenJournalLen)
+      .(isFrozen := true)
+      .(syncReqs := SyncReqs3to2(cm.syncReqs))
+  }
+
+  lemma freezeCorrect(k: Constants, cm: CM)
+  requires CommitterModel.WF(cm)
+  requires cm.superblockWrite.None?
+
+  // Mostly we'll probably just do this with cm.frozenLoc == None
+  // but more generally we can do it whenever we have:
+  requires cm.status == StatusReady
+  requires cm.frozenLoc != Some(cm.superblock.indirectionTableLoc)
+  requires JournalistModel.I(cm.journalist).replayJournal == []
+
+  ensures var cm' := freeze(k, cm);
+    && CommitterModel.WF(cm')
+    && JC.Next(Ik(k).jc,
+        CommitterModel.I(cm),
+        CommitterModel.I(cm'),
+        JournalDisk.NoDiskOp,
+        FreezeOp)
+  {
+    reveal_freeze();
+    var cm' := freeze(k, cm);
+    SyncReqs3to2Correct(cm.syncReqs);
+
+    assert JC.Freeze(Ik(k).jc,
+        CommitterModel.I(cm),
+        CommitterModel.I(cm'),
+        JournalDisk.NoDiskOp,
+        FreezeOp);
+    assert JC.NextStep(Ik(k).jc,
+        CommitterModel.I(cm),
+        CommitterModel.I(cm'),
+        JournalDisk.NoDiskOp,
+        FreezeOp,
+        JC.FreezeStep);
+  }
+
+  function {:opaque} receiveFrozenLoc(
+      k: Constants, cm: CM, loc: Location) : (cm': CM)
+  {
+    cm.(frozenLoc := Some(loc))
+  }
+
+  lemma receiveFrozenLocCorrect(k: Constants, cm: CM, loc: Location)
+  requires CommitterModel.WF(cm)
+  requires cm.status == StatusReady
+  requires cm.isFrozen
+  requires !cm.frozenLoc.Some?
+  requires ValidIndirectionTableLocation(loc)
+
+  ensures var cm' := receiveFrozenLoc(k, cm, loc);
+    && CommitterModel.WF(cm')
+    && JC.Next(Ik(k).jc,
+        CommitterModel.I(cm),
+        CommitterModel.I(cm'),
+        JournalDisk.NoDiskOp,
+        SendFrozenLocOp(loc))
+  {
+    reveal_receiveFrozenLoc();
+    var cm' := receiveFrozenLoc(k, cm, loc);
+    assert JC.ReceiveFrozenLoc(Ik(k).jc,
+        CommitterModel.I(cm),
+        CommitterModel.I(cm'),
+        JournalDisk.NoDiskOp,
+        SendFrozenLocOp(loc));
+    assert JC.NextStep(Ik(k).jc,
+        CommitterModel.I(cm),
+        CommitterModel.I(cm'),
+        JournalDisk.NoDiskOp,
+        SendFrozenLocOp(loc),
+        JC.ReceiveFrozenLocStep);
+  }
+
+  // == pushSync ==
+
+  function {:opaque} freeId<A>(syncReqs: MutableMapModel.LinearHashMap<A>) : (id: uint64)
+  requires MutableMapModel.Inv(syncReqs)
+  ensures id != 0 ==> id !in syncReqs.contents
+  {
+    var maxId := MutableMapModel.MaxKey(syncReqs);
+    if maxId == 0xffff_ffff_ffff_ffff then (
+      0
+    ) else (
+      maxId + 1
+    )
+  }
+
+  function pushSync(k: Constants, cm: CM) : (CM, uint64)
+  requires CommitterModel.WF(cm)
+  {
+    var id := freeId(cm.syncReqs);
+    if id == 0 || cm.syncReqs.count as int >= 0x1_0000_0000_0000_0000 / 8 then (
+      (cm, 0)
+    ) else (
+      var cm' := cm.(syncReqs := MutableMapModel.Insert(cm.syncReqs, id, JC.State3));
+      (cm', id)
+    )
+  }
+
+  lemma pushSyncCorrect(k: Constants, cm: CM)
+  requires CommitterModel.WF(cm)
+
+  ensures var (cm', id) := pushSync(k, cm);
+    && CommitterModel.WF(cm')
+    && JC.Next(Ik(k).jc,
+        CommitterModel.I(cm),
+        CommitterModel.I(cm'),
+        JournalDisk.NoDiskOp,
+        if id == 0 then JournalInternalOp else PushSyncOp(id as int))
+  {
+    var (cm', id) := pushSync(k, cm);
+    if id == 0 || cm.syncReqs.count as int >= 0x1_0000_0000_0000_0000 / 8 {
+      assert JC.NoOp(Ik(k).jc,
+          CommitterModel.I(cm),
+          CommitterModel.I(cm'),
+          JournalDisk.NoDiskOp,
+          JournalInternalOp);
+      assert JC.NextStep(Ik(k).jc,
+          CommitterModel.I(cm),
+          CommitterModel.I(cm'),
+          JournalDisk.NoDiskOp,
+          JournalInternalOp,
+          JC.NoOpStep);
+    } else {
+      assert JC.PushSyncReq(Ik(k).jc,
+          CommitterModel.I(cm),
+          CommitterModel.I(cm'),
+          JournalDisk.NoDiskOp,
+          PushSyncOp(id as int), id);
+      assert JC.NextStep(Ik(k).jc,
+          CommitterModel.I(cm),
+          CommitterModel.I(cm'),
+          JournalDisk.NoDiskOp,
+          PushSyncOp(id as int),
+          JC.PushSyncReqStep(id));
+    }
+  }
+
+  // == popSync ==
+
+  function {:opaque} popSync(k: Constants, cm: CM, id: uint64) : (cm' : CM)
+  requires CommitterModel.WF(cm)
+  {
+    cm.(syncReqs := MutableMapModel.Remove(cm.syncReqs, id))
+  }
+
+  lemma popSyncCorrect(k: Constants, cm: CM, id: uint64)
+  requires CommitterModel.WF(cm)
+  requires id in cm.syncReqs.contents
+  requires cm.syncReqs.contents[id] == JC.State1
+  ensures var cm' := popSync(k, cm, id);
+    && CommitterModel.WF(cm')
+    && JC.Next(Ik(k).jc,
+        CommitterModel.I(cm),
+        CommitterModel.I(cm'),
+        JournalDisk.NoDiskOp,
+        PopSyncOp(id as int))
+  {
+    var cm' := popSync(k, cm, id);
+    reveal_popSync();
+    assert JC.PopSyncReq(Ik(k).jc,
+        CommitterModel.I(cm),
+        CommitterModel.I(cm'),
+        JournalDisk.NoDiskOp,
+        PopSyncOp(id as int), id);
+    assert JC.NextStep(Ik(k).jc,
+        CommitterModel.I(cm),
+        CommitterModel.I(cm'),
+        JournalDisk.NoDiskOp,
+        PopSyncOp(id as int),
+        JC.PopSyncReqStep(id));
+  }
+
+  // == AdvanceLog ==
+
+  predicate {:opaque} tryAdvanceLog(k: Constants, cm: CM, io: IO,
+      cm': CM, io': IO)
+  requires CommitterModel.WF(cm)
+  requires io.IOInit?
+  {
+    var hasFrozen := JournalistModel.hasFrozenJournal(cm.journalist);
+    var hasInMem := JournalistModel.hasInMemoryJournal(cm.journalist);
+    if cm.superblockWrite.None? then (
+      if hasFrozen || hasInMem then (
+        (cm', io') == WriteOutJournal(k, cm, io)
+      ) else if cm.outstandingJournalWrites == {} then (
+        writeOutSuperblockAdvanceLog(k, cm, io, cm', io')
+      ) else (
+        && cm' == cm
+        && io' == io
+      )
+    ) else (
+      && cm' == cm
+      && io' == io
+    )
+  }
+
+  lemma tryAdvanceLogCorrect(k: Constants, cm: CM, io: IO,
+      cm': CM, io': IO)
+  requires CommitterModel.Inv(cm)
+  requires io.IOInit?
+  requires cm.status.StatusReady?
+  requires tryAdvanceLog(k, cm, io, cm', io')
+  ensures CommitterModel.WF(cm')
+  ensures ValidDiskOp(diskOp(io'))
+  ensures IDiskOp(diskOp(io')).bdop.NoDiskOp?
+  ensures JC.Next(Ik(k).jc,
+        CommitterModel.I(cm),
+        CommitterModel.I(cm'),
+        IDiskOp(diskOp(io')).jdop,
+        JournalInternalOp)
+  {
+    reveal_tryAdvanceLog();
+    var hasFrozen := JournalistModel.hasFrozenJournal(cm.journalist);
+    var hasInMem := JournalistModel.hasInMemoryJournal(cm.journalist);
+    if cm.superblockWrite.None? {
+      if hasFrozen || hasInMem {
+        WriteOutJournalCorrect(k, cm, io);
+      } else if (cm.outstandingJournalWrites == {}) {
+        writeOutSuperblockAdvanceLogCorrect(k, cm, io, cm', io');
+      } else {
+        assert JC.NoOp(Ik(k).jc, CommitterModel.I(cm), CommitterModel.I(cm'), JournalDisk.NoDiskOp, JournalInternalOp);
+        assert JC.NextStep(Ik(k).jc, CommitterModel.I(cm), CommitterModel.I(cm'), JournalDisk.NoDiskOp, JournalInternalOp, JC.NoOpStep);
+      }
+    } else {
+      assert JC.NoOp(Ik(k).jc, CommitterModel.I(cm), CommitterModel.I(cm'), JournalDisk.NoDiskOp, JournalInternalOp);
+      assert JC.NextStep(Ik(k).jc, CommitterModel.I(cm), CommitterModel.I(cm'), JournalDisk.NoDiskOp, JournalInternalOp, JC.NoOpStep);
+    }
+  }
+
+  predicate {:opaque} tryAdvanceLocation(k: Constants, cm: CM, io: IO,
+      cm': CM, io': IO)
+  requires CommitterModel.Inv(cm)
+  requires io.IOInit?
+  requires cm.status == StatusReady
+  requires cm.frozenLoc.Some?
+  {
+    var hasFrozen := JournalistModel.hasFrozenJournal(cm.journalist);
+    var hasInMem := JournalistModel.hasInMemoryJournal(cm.journalist);
+    if cm.superblockWrite.None? then (
+      if hasFrozen || hasInMem then (
+        (cm', io') == WriteOutJournal(k, cm, io)
+      ) else if cm.outstandingJournalWrites == {} then (
+        writeOutSuperblockAdvanceLocation(k, cm, io, cm', io')
+      ) else (
+        && cm' == cm
+        && io' == io
+      )
+    ) else (
+      && cm' == cm
+      && io' == io
+    )
+  }
+
+  lemma tryAdvanceLocationCorrect(k: Constants, cm: CM, io: IO,
+      cm': CM, io': IO)
+  requires CommitterModel.Inv(cm)
+  requires io.IOInit?
+  requires cm.status.StatusReady?
+  requires cm.frozenLoc.Some?
+  requires tryAdvanceLocation(k, cm, io, cm', io')
+  ensures CommitterModel.WF(cm')
+  ensures ValidDiskOp(diskOp(io'))
+  ensures IDiskOp(diskOp(io')).bdop.NoDiskOp?
+  ensures JC.Next(Ik(k).jc,
+        CommitterModel.I(cm),
+        CommitterModel.I(cm'),
+        IDiskOp(diskOp(io')).jdop,
+        JournalInternalOp)
+  {
+    reveal_tryAdvanceLocation();
+    var hasFrozen := JournalistModel.hasFrozenJournal(cm.journalist);
+    var hasInMem := JournalistModel.hasInMemoryJournal(cm.journalist);
+    if cm.superblockWrite.None? {
+      if hasFrozen || hasInMem {
+        WriteOutJournalCorrect(k, cm, io);
+      } else if (cm.outstandingJournalWrites == {}) {
+        writeOutSuperblockAdvanceLocationCorrect(k, cm, io, cm', io');
+      } else {
+        assert JC.NoOp(Ik(k).jc, CommitterModel.I(cm), CommitterModel.I(cm'), JournalDisk.NoDiskOp, JournalInternalOp);
+        assert JC.NextStep(Ik(k).jc, CommitterModel.I(cm), CommitterModel.I(cm'), JournalDisk.NoDiskOp, JournalInternalOp, JC.NoOpStep);
+      }
+    } else {
+      assert JC.NoOp(Ik(k).jc, CommitterModel.I(cm), CommitterModel.I(cm'), JournalDisk.NoDiskOp, JournalInternalOp);
+      assert JC.NextStep(Ik(k).jc, CommitterModel.I(cm), CommitterModel.I(cm'), JournalDisk.NoDiskOp, JournalInternalOp, JC.NoOpStep);
+    }
+  }
+
+  function {:opaque} writeBackSuperblockResp(
+      k: Constants, cm: CommitterModel.CM) : CommitterModel.CM
+  requires CommitterModel.Inv(cm)
+  {
+    if cm.status.StatusReady? &&
+        cm.commitStatus.CommitAdvanceLocation? then (
+      cm.(superblockWrite := None)
+        .(superblock := cm.newSuperblock.value)
+        .(newSuperblock := None)
+        .(whichSuperblock := if cm.whichSuperblock == 0 then 1 else 0)
+        .(syncReqs := SyncReqs2to1(cm.syncReqs))
+        .(journalist :=
+            JournalistModel.updateWrittenJournalLen(
+              cm.journalist,
+              JournalistModel.getWrittenJournalLen(cm.journalist)
+                - cm.frozenJournalPosition
+            )
+         )
+        .(frozenJournalPosition := 0)
+        .(frozenLoc := None)
+        .(isFrozen := false)
+        .(commitStatus := JC.CommitNone)
+    )
+    else if cm.status.StatusReady? &&
+        cm.commitStatus.CommitAdvanceLog? then (
+      cm.(superblockWrite := None)
+        .(superblock := cm.newSuperblock.value)
+        .(newSuperblock := None)
+        .(whichSuperblock := if cm.whichSuperblock == 0 then 1 else 0)
+        .(syncReqs := SyncReqs2to1(cm.syncReqs))
+        .(commitStatus := JC.CommitNone)
+    )
+    else (
+      cm
+    )
+  }
+
+  lemma writeBackSuperblockRespCorrect(
+      k: Constants, cm: CommitterModel.CM, io: IO)
+  requires CommitterModel.Inv(cm)
+  requires ValidDiskOp(diskOp(io))
+  requires IDiskOp(diskOp(io)).jdop.RespWriteSuperblockOp?
+  requires Some(io.id) == cm.superblockWrite
+  ensures var cm' := writeBackSuperblockResp(k, cm);
+    && CommitterModel.WF(cm')
+    && JC.Next(Ik(k).jc,
+        CommitterModel.I(cm),
+        CommitterModel.I(cm'),
+        IDiskOp(diskOp(io)).jdop,
+        if cm.status.StatusReady? && cm.commitStatus.CommitAdvanceLocation? then CleanUpOp else JournalInternalOp
+    )
+  {
+    reveal_writeBackSuperblockResp();
+    var cm' := writeBackSuperblockResp(k, cm);
+    SyncReqs2to1Correct(cm.syncReqs);
+    if cm.status.StatusReady? &&
+        cm.commitStatus.CommitAdvanceLocation? {
+      assert JC.WriteBackSuperblockResp(Ik(k).jc,
+          CommitterModel.I(cm),
+          CommitterModel.I(cm'),
+          IDiskOp(diskOp(io)).jdop,
+          CleanUpOp);
+      assert JC.NextStep(Ik(k).jc,
+          CommitterModel.I(cm),
+          CommitterModel.I(cm'),
+          IDiskOp(diskOp(io)).jdop,
+          CleanUpOp,
+          JC.WriteBackSuperblockRespStep);
+    }
+    else if cm.status.StatusReady? &&
+        cm.commitStatus.CommitAdvanceLog? {
+      assert JC.WriteBackSuperblockResp(Ik(k).jc,
+          CommitterModel.I(cm),
+          CommitterModel.I(cm'),
+          IDiskOp(diskOp(io)).jdop,
+          JournalInternalOp);
+      assert JC.NextStep(Ik(k).jc,
+          CommitterModel.I(cm),
+          CommitterModel.I(cm'),
+          IDiskOp(diskOp(io)).jdop,
+          JournalInternalOp,
+          JC.WriteBackSuperblockRespStep);
+    }
+    else {
+      assert JC.NoOp(Ik(k).jc,
+          CommitterModel.I(cm),
+          CommitterModel.I(cm'),
+          IDiskOp(diskOp(io)).jdop,
+          JournalInternalOp);
+      assert JC.NextStep(Ik(k).jc,
+          CommitterModel.I(cm),
+          CommitterModel.I(cm'),
+          IDiskOp(diskOp(io)).jdop,
+          JournalInternalOp,
+          JC.NoOpStep);
+    }
+  }
+}
