Impl/DiskOpModel.i.dfy
@@ -1,0 +1,38 @@
+include "../ByteBlockCacheSystem/AsyncDiskModel.s.dfy"
+include "../BlockCacheSystem/BlockJournalCache.i.dfy"
+
+module DiskOpModel {
+  import D = AsyncDisk
+  import opened NativeTypes
+  import BJC = BlockJournalCache
+  import BC = BlockCache
+  import JC = JournalCache
+
+  datatype Constants = Constants()
+
+  function Ik(k: Constants) : BJC.Constants
+  {
+    BJC.Constants(BC.Constants(), JC.Constants())
+  }
+
+  // Functional model of the DiskIOHandler
+
+  datatype IO =
+    | IOInit(id: uint64, id2: uint64)
+    | IOReqRead(id: uint64, reqRead: D.ReqRead)
+    | IOReqWrite(id: uint64, reqWrite: D.ReqWrite)
+    | IOReqWrite2(id: uint64, id2: uint64, reqWrite1: D.ReqWrite, reqWrite2: D.ReqWrite)
+    | IORespRead(id: uint64, respRead: D.RespRead)
+    | IORespWrite(id: uint64, respWrite: D.RespWrite)
+
+  function diskOp(io: IO) : D.DiskOp {
+    match io {
+      case IOInit(id, id2) => D.NoDiskOp
+      case IOReqRead(id, reqRead) => D.ReqReadOp(id, reqRead)
+      case IOReqWrite(id, reqWrite) => D.ReqWriteOp(id, reqWrite)
+      case IOReqWrite2(id1, id2, reqWrite1, reqWrite2) => D.ReqWrite2Op(id1, id2, reqWrite1, reqWrite2)
+      case IORespRead(id, respRead) => D.RespReadOp(id, respRead)
+      case IORespWrite(id, respWrite) => D.RespWriteOp(id, respWrite)
+    }
+  }
+}
