Impl/JournalistMarshallingImpl.i.dfy
@@ -1,0 +1,164 @@
+include "../ByteBlockCacheSystem/JournalBytes.i.dfy"
+include "../BlockCacheSystem/DiskLayout.i.dfy"
+include "JournalistMarshallingModel.i.dfy"
+include "../lib/Base/NativeArrays.s.dfy"
+
+module JournalistMarshallingImpl {
+  import opened JournalRanges`Internal
+  import opened JournalBytes
+  import opened Journal
+  import opened DiskLayout
+  import opened NativeTypes
+  import opened Options
+  import opened Sequences
+  import opened Crypto
+  import opened NativePackedInts
+  import opened PackedIntsLib
+  import NativeArrays
+
+  import JournalistMarshallingModel
+
+  ///// Marshalling
+
+  method Splice(buf: array<byte>, start: uint64, ins: seq<byte>)
+  requires |ins| < 0x1_0000_0000_0000_0000
+  requires buf.Length < 0x1_0000_0000_0000_0000
+  requires 0 <= start
+  requires start as int + |ins| <= buf.Length
+  modifies buf
+  ensures buf[..] == JournalistMarshallingModel.splice(
+      old(buf[..]), start, ins);
+  {
+    JournalistMarshallingModel.reveal_splice();
+    NativeArrays.CopySeqIntoArray(ins, 0, buf, start,
+        |ins| as uint64);
+  }
+
+  method WriteOnto(buf: array<byte>, numBlocks: uint64, start: uint64, bytes: seq<byte>)
+  requires buf.Length == 4096 * numBlocks as int
+  requires numBlocks <= NumJournalBlocks()
+  requires |bytes| <= 4064
+  requires 0 <= start as int <= start as int + |bytes| <= 4064 * numBlocks as int
+  modifies buf
+  ensures buf[..] == JournalistMarshallingModel.writeOnto(
+      old(buf[..]), numBlocks, start, bytes)
+  {
+    JournalistMarshallingModel.reveal_writeOnto();
+    
+    if |bytes| as uint64 > 0 {
+      var block: uint64 := start / 4064;
+      var idx: uint64 := start % 4064;
+      if idx + |bytes| as uint64 <= 4064 {
+        Splice(buf, block * 4096 + 32 + idx, bytes);
+      } else {
+        Splice(buf, block * 4096 + 32 + idx, bytes[.. 4064 - idx]);
+        Splice(buf, (block + 1) * 4096 + 32, bytes[4064 - idx ..]);
+      }
+    }
+  }
+
+  method WriteIntOnto(buf: array<byte>, numBlocks: uint64, start: uint64, val: uint32)
+  requires buf.Length == 4096 * numBlocks as int
+  requires numBlocks <= NumJournalBlocks()
+  requires 0 <= start
+  requires start as int + 4 <= numBlocks as int * 4064
+  modifies buf
+  ensures buf[..] == JournalistMarshallingModel.writeIntOnto(
+      old(buf[..]), numBlocks, start, val)
+  {
+    JournalistMarshallingModel.reveal_writeIntOnto();
+    WriteOnto(buf, numBlocks, start,
+        pack_LittleEndian_Uint32(val));
+  }
+
+  method WriteHeader(buf: array<byte>, numBlocks: uint64, len: uint64)
+  requires buf.Length == 4096 * numBlocks as int
+  requires 1 <= numBlocks <= NumJournalBlocks()
+  requires len <= 0xffff_ffff
+  modifies buf
+  ensures buf[..] == JournalistMarshallingModel.writeHeader(
+      old(buf[..]), numBlocks, len)
+  {
+    WriteIntOnto(buf, numBlocks, 0, len as uint32);
+    WriteIntOnto(buf, numBlocks, 4, numBlocks as uint32);
+  }
+
+  method WriteJournalEntries(
+      buf: array<byte>, numBlocks: uint64, idx: uint64,
+      entries: array<JournalEntry>, start: uint64, len: uint64)
+  requires buf.Length == 4096 * numBlocks as int
+  requires numBlocks <= NumJournalBlocks()
+  requires 0 <= start as int < entries.Length
+  requires 0 <= len as int <= entries.Length
+  requires entries.Length < 0xfff_ffff_ffff_ffff
+  requires idx as int + SumJournalEntries(JournalistMarshallingModel.cyclicSlice(entries[..], start, len)) <= 4064 * numBlocks as int
+  modifies buf
+  decreases len
+  ensures buf[..] == JournalistMarshallingModel.writeJournalEntries(
+      old(buf[..]), numBlocks, idx, entries[..], start, len)
+  {
+    JournalistMarshallingModel.reveal_writeJournalEntries();
+    if len != 0 {
+      var start' := if start+1 == entries.Length as uint64 then 0 else start+1;
+      JournalistMarshallingModel.
+          lemma_cyclicRange_popFront_Sum(entries[..], start, len);
+
+      WriteIntOnto(buf, numBlocks, idx, |entries[start].key| as uint32);
+      var idx1 := idx + 4;
+      WriteOnto(buf, numBlocks, idx1, entries[start].key);
+      var idx2 := idx1 + |entries[start].key| as uint64;
+      WriteIntOnto(buf, numBlocks, idx2, |entries[start].value| as uint32);
+      var idx3 := idx2 + 4;
+      WriteOnto(buf, numBlocks, idx3, entries[start].value);
+      var idx4 := idx3 + |entries[start].value| as uint64;
+      WriteJournalEntries(buf, numBlocks, idx4, entries, start', len - 1);
+    }
+  }
+
+  method FillInChecksums(buf: array<byte>, numBlocks: uint64, i: uint64)
+  requires buf.Length == numBlocks as int * 4096
+  requires numBlocks <= NumJournalBlocks()
+  requires 0 <= i <= numBlocks
+  modifies buf
+  decreases numBlocks - i
+  ensures buf[..] == JournalistMarshallingModel.fillInChecksums(
+      old(buf[..]), numBlocks, i)
+  {
+    JournalistMarshallingModel.reveal_fillInChecksums();
+    if i != numBlocks {
+      var c := Crc32CArray(buf, 4096*i + 32, 4064);
+      NativeArrays.CopySeqIntoArray(c, 0, buf, 4096*i, 32);
+      assert buf[..] == JournalistMarshallingModel.splice(
+          old(buf[..]), 4096*i, c) by {
+        JournalistMarshallingModel.reveal_splice();
+      }
+      FillInChecksums(buf, numBlocks, i+1);
+    }
+  }
+
+  method MarshallJournalEntries(
+      entries: array<JournalEntry>,
+      start: uint64, len: uint64, numBlocks: uint64)
+  returns (res: seq<byte>)
+  requires 0 <= start as int < entries.Length
+  requires 0 <= len as int <= entries.Length
+  requires entries.Length <= 0xffff_ffff
+  requires WeightJournalEntries(JournalistMarshallingModel.cyclicSlice(entries[..], start, len)) <= 4064 * numBlocks as int
+  requires 1 <= numBlocks <= NumJournalBlocks()
+
+  ensures res == JournalistMarshallingModel.marshallJournalEntries(
+      entries[..], start, len, numBlocks)
+  {
+    reveal_WeightJournalEntries();
+    JournalistMarshallingModel.reveal_marshallJournalEntries();
+
+    var buf := NativeArrays.newArrayFill(numBlocks * 4096, 0);
+    assert buf[..] == fill((numBlocks * 4096) as int, 0);
+    WriteHeader(buf, numBlocks, len);
+    WriteJournalEntries(buf, numBlocks, 8, entries, start, len);
+    FillInChecksums(buf, numBlocks, 0);
+
+    return buf[..];
+  }
+
+}
