Impl/JournalistModel.i.dfy
@@ -1,0 +1,370 @@
+include "../ByteBlockCacheSystem/JournalBytes.i.dfy"
+include "../BlockCacheSystem/DiskLayout.i.dfy"
+include "JournalistMarshallingModel.i.dfy"
+
+module JournalistModel {
+  import opened DiskLayout
+  import opened NativeTypes
+  import opened Options
+  import opened Sequences
+
+  import opened JournalRanges`Internal
+  import opened JournalBytes
+  import opened Journal
+  import opened JournalistMarshallingModel
+
+  datatype JournalInfo = JournalInfo(
+    inMemoryJournalFrozen: seq<JournalEntry>,
+    inMemoryJournal: seq<JournalEntry>,
+    replayJournal: seq<JournalEntry>,
+
+    journalFront: Option<JournalRange>,
+    journalBack: Option<JournalRange>,
+
+    ghost writtenJournalLen: int
+  )
+
+  datatype JournalistModel = JournalistModel(
+    journalEntries: seq<JournalEntry>,
+    start: uint64,
+    len1: uint64,
+    len2: uint64,
+
+    replayJournal: seq<JournalEntry>,
+    replayIdx: uint64,
+
+    journalFront: Option<seq<byte>>,
+    journalBack: Option<seq<byte>>,
+    
+    // number of blocks already written on disk:
+    writtenJournalBlocks: uint64,
+    // number of *blocks* of inMemoryJournalFrozen:
+    frozenJournalBlocks: uint64,
+    // number of *bytes* of inMemoryJournal:
+    inMemoryWeight: uint64
+  )
+
+  function method Len() : uint64 { 1048576 }
+
+  function method basic_mod(x: uint64) : uint64
+  {
+    if x >= Len() then x - Len() else x
+  }
+
+  predicate WF(jm: JournalistModel)
+  {
+    && |jm.journalEntries| == Len() as int
+    && 0 <= jm.start < Len()
+    && 0 <= jm.len1 <= Len()
+    && 0 <= jm.len2 <= Len()
+    && 0 <= jm.len1 + jm.len2 <= Len()
+    && 0 <= jm.replayIdx as int <= |jm.replayJournal| <= Len() as int
+    && (jm.journalFront.Some? ==>
+        JournalRangeOfByteSeq(jm.journalFront.value).Some?)
+    && (jm.journalBack.Some? ==>
+        JournalRangeOfByteSeq(jm.journalBack.value).Some?)
+    && 0 <= jm.writtenJournalBlocks <= NumJournalBlocks()
+    && 0 <= jm.frozenJournalBlocks <= NumJournalBlocks()
+    && 0 <= jm.inMemoryWeight <= NumJournalBlocks() * 4096
+  }
+
+  function IJournalRead(j: Option<seq<byte>>) : Option<JournalRange>
+  requires j.Some? ==> JournalRangeOfByteSeq(j.value).Some?
+  {
+    if j.Some? then JournalRangeOfByteSeq(j.value) else None
+  }
+
+  function start(jm: JournalistModel) : uint64
+  {
+    jm.start
+  }
+
+  function mid(jm: JournalistModel) : uint64
+  requires jm.start < Len()
+  requires jm.len1 <= Len()
+  {
+    basic_mod(jm.start + jm.len1)
+  }
+
+  function end(jm: JournalistModel) : uint64
+  requires jm.start < Len()
+  requires jm.len1 <= Len()
+  requires jm.len2 <= Len()
+  {
+    basic_mod(jm.start + jm.len1 + jm.len2)
+  }
+
+  function InMemoryJournalFrozen(jm: JournalistModel) : seq<JournalEntry>
+  requires WF(jm)
+  {
+    cyclicSlice(jm.journalEntries, start(jm), jm.len1)
+  }
+
+  function InMemoryJournal(jm: JournalistModel) : seq<JournalEntry>
+  requires WF(jm)
+  {
+    cyclicSlice(jm.journalEntries, mid(jm), jm.len2)
+  }
+
+  function ReplayJournal(jm: JournalistModel) : seq<JournalEntry>
+  requires 0 <= jm.replayIdx as int <= |jm.replayJournal|
+  {
+    jm.replayJournal[jm.replayIdx..]
+  }
+
+  function JournalFrontRead(jm: JournalistModel) : Option<JournalRange>
+  requires WF(jm)
+  {
+    IJournalRead(jm.journalFront)
+  }
+
+  function JournalBackRead(jm: JournalistModel) : Option<JournalRange>
+  requires WF(jm)
+  {
+    IJournalRead(jm.journalBack)
+  }
+
+  function WrittenJournalLen(jm: JournalistModel) : int
+  {
+    jm.writtenJournalBlocks as int
+  }
+
+  function Iprivate(jm: JournalistModel) : JournalInfo
+  requires WF(jm)
+  {
+    JournalInfo(
+      InMemoryJournalFrozen(jm),
+      InMemoryJournal(jm),
+      ReplayJournal(jm),
+      JournalFrontRead(jm),
+      JournalBackRead(jm),
+      WrittenJournalLen(jm)
+    )
+  }
+
+  protected function I(jm: JournalistModel) : JournalInfo
+  requires WF(jm)
+  {
+    Iprivate(jm)
+  }
+
+  lemma reveal_I(jm: JournalistModel)
+  requires WF(jm)
+  ensures I(jm) == Iprivate(jm)
+
+  predicate Inv(jm: JournalistModel)
+  {
+    && WF(jm)
+    && (jm.writtenJournalBlocks + jm.frozenJournalBlocks) * 4064 +
+        jm.inMemoryWeight <= 4064 * NumJournalBlocks()
+    && WeightJournalEntries(InMemoryJournalFrozen(jm)) <= jm.frozenJournalBlocks as int * 4064
+    && WeightJournalEntries(InMemoryJournal(jm)) == jm.inMemoryWeight as int
+  }
+
+  //// Journalist operations
+
+  function {:opaque} JournalistConstructor() : (jm : JournalistModel)
+  ensures Inv(jm)
+  ensures I(jm).inMemoryJournalFrozen == []
+  ensures I(jm).inMemoryJournal == []
+  ensures I(jm).replayJournal == []
+  ensures I(jm).journalFront == None
+  ensures I(jm).journalBack == None
+  ensures I(jm).writtenJournalLen == 0
+  {
+    reveal_cyclicSlice();
+    reveal_WeightJournalEntries();
+    JournalistModel(
+        fill(Len() as int, JournalInsert([], [])), // fill with dummies
+        0, 0, 0, [], 0, None, None, 0, 0, 0)
+  }
+
+  function {:opaque} hasFrozenJournal(jm: JournalistModel) : (b: bool)
+  requires Inv(jm)
+  ensures b == (I(jm).inMemoryJournalFrozen != [])
+  {
+    jm.len1 != 0
+  }
+
+  function {:opaque} hasInMemoryJournal(jm: JournalistModel) : (b: bool)
+  requires Inv(jm)
+  ensures b == (I(jm).inMemoryJournal != [])
+  {
+    jm.len2 != 0
+  }
+
+  function {:opaque} packageFrozenJournal(jm: JournalistModel)
+      : (res : (JournalistModel, seq<byte>))
+  requires Inv(jm)
+  requires I(jm).inMemoryJournalFrozen != []
+  ensures var (jm', s) := res;
+    && Inv(jm')
+    && JournalRangeOfByteSeq(s).Some?
+    && parseJournalRange(JournalRangeOfByteSeq(s).value) == Some(I(jm).inMemoryJournalFrozen)
+    && I(jm') == I(jm)
+          .(inMemoryJournalFrozen := [])
+          .(writtenJournalLen := I(jm).writtenJournalLen
+                + |JournalRangeOfByteSeq(s).value|)
+    && |JournalRangeOfByteSeq(s).value| + I(jm).writtenJournalLen as int
+        <= NumJournalBlocks() as int
+  {
+    reveal_WeightJournalEntries();
+    var s := marshallJournalEntries(jm.journalEntries, jm.start, jm.len1, jm.frozenJournalBlocks);
+    var jm' := jm.(start := basic_mod(jm.start + jm.len1))
+                 .(len1 := 0)
+                 .(frozenJournalBlocks := 0)
+                 .(writtenJournalBlocks := jm.writtenJournalBlocks + jm.frozenJournalBlocks);
+    (jm', s)
+  }
+
+  function {:opaque} packageInMemoryJournal(jm: JournalistModel)
+      : (res : (JournalistModel, seq<byte>))
+  requires Inv(jm)
+  requires I(jm).inMemoryJournalFrozen == []
+  requires I(jm).inMemoryJournal != []
+  ensures var (jm', s) := res;
+    && Inv(jm')
+    && JournalRangeOfByteSeq(s).Some?
+    && parseJournalRange(JournalRangeOfByteSeq(s).value) == Some(I(jm).inMemoryJournal)
+    && I(jm') == I(jm)
+          .(inMemoryJournal := [])
+          .(writtenJournalLen := I(jm).writtenJournalLen
+                + |JournalRangeOfByteSeq(s).value|)
+    && |JournalRangeOfByteSeq(s).value| + I(jm).writtenJournalLen as int
+        <= NumJournalBlocks() as int
+  {
+    reveal_WeightJournalEntries();
+    var numBlocks := (jm.inMemoryWeight + 4064 - 1) / 4064;
+    var s := marshallJournalEntries(jm.journalEntries, jm.start, jm.len2, numBlocks);
+    var jm' := jm.(start := 0)
+                 .(len2 := 0)
+                 .(inMemoryWeight := 0)
+                 .(writtenJournalBlocks := jm.writtenJournalBlocks + numBlocks);
+    (jm', s)
+  }
+
+  function getWrittenJournalLen(jm: JournalistModel)
+      : (len : uint64)
+  requires Inv(jm)
+  ensures len as int == I(jm).writtenJournalLen
+  {
+    jm.writtenJournalBlocks    
+  }
+
+  function setWrittenJournalLen(jm: JournalistModel, len: uint64)
+      : (jm' : JournalistModel)
+  requires Inv(jm)
+  requires I(jm).inMemoryJournal == []
+  requires I(jm).inMemoryJournalFrozen == []
+  requires 0 <= len <= NumJournalBlocks()
+  ensures Inv(jm')
+  ensures I(jm') == I(jm).(writtenJournalLen := len as int)
+  {
+    reveal_WeightJournalEntries();
+    jm.(writtenJournalBlocks := len)
+      .(frozenJournalBlocks := 0)
+  }
+
+  function updateWrittenJournalLen(jm: JournalistModel, len: uint64)
+      : (jm' : JournalistModel)
+  requires Inv(jm)
+  requires len as int <= I(jm).writtenJournalLen
+  ensures Inv(jm')
+  ensures I(jm') == I(jm).(writtenJournalLen := len as int)
+  {
+    reveal_WeightJournalEntries();
+    jm.(writtenJournalBlocks := len)
+  }
+
+  /*lemma roundUpOkay(a: int, b: int)
+  requires a <= 4064 * b
+  ensures ((a + 4064 - 1) / 4064) * 4064 <= 4064 * b
+  {
+  }*/
+
+  function {:opaque} freeze(jm: JournalistModel) : (jm' : JournalistModel)
+  requires Inv(jm)
+  ensures
+    && Inv(jm')
+    && I(jm') == I(jm)
+          .(inMemoryJournal := [])
+          .(inMemoryJournalFrozen :=
+              I(jm).inMemoryJournalFrozen + I(jm).inMemoryJournal)
+  {
+    var jm' := jm.(len1 := jm.len1 + jm.len2)
+      .(len2 := 0)
+      .(frozenJournalBlocks := jm.frozenJournalBlocks + (jm.inMemoryWeight + 4064 - 1) / 4064)
+      .(inMemoryWeight := 0);
+
+    reveal_WeightJournalEntries();
+    assert I(jm').inMemoryJournalFrozen ==
+        I(jm).inMemoryJournalFrozen + I(jm).inMemoryJournal
+      by { reveal_cyclicSlice(); }
+
+    WeightJournalEntriesSum(I(jm).inMemoryJournalFrozen, I(jm).inMemoryJournal);
+    //roundUpOkay(jm.inMemoryWeight as int,
+    //  NumJournalBlocks() as int - (jm.writtenJournalBlocks + jm.frozenJournalBlocks) as int);
+
+    jm'
+  }
+
+  predicate {:opaque} canAppend(jm: JournalistModel, je: JournalEntry)
+  requires Inv(jm)
+  {
+    4064 * (jm.writtenJournalBlocks + jm.frozenJournalBlocks)
+      + jm.inMemoryWeight
+      + WeightJournalEntry(je) as uint64
+      + (if jm.len2 == 0 then 8 else 0)
+        <= 4064 * NumJournalBlocks()
+  }
+
+  lemma lemma_weight_append(a: seq<JournalEntry>, je: JournalEntry)
+  ensures |a| == 0 ==> WeightJournalEntries(a + [je])
+      == WeightJournalEntries(a) + WeightJournalEntry(je) + 8
+  ensures |a| > 0 ==> WeightJournalEntries(a + [je])
+      == WeightJournalEntries(a) + WeightJournalEntry(je)
+  {
+    assert DropLast(a + [je]) == a;
+    assert Last(a + [je]) == je;
+    reveal_WeightJournalEntries();
+    if |a| == 0 {
+      assert WeightJournalEntries(a + [je])
+          == 8 + SumJournalEntries(a) + WeightJournalEntry(je)
+          == 8 + SumJournalEntries([]) + WeightJournalEntry(je)
+          == 8 + WeightJournalEntry(je);
+      assert WeightJournalEntries(a) == 0;
+    }
+  }
+
+  function {:opaque} append(jm: JournalistModel, je: JournalEntry) : (jm' : JournalistModel)
+  requires Inv(jm)
+  requires canAppend(jm, je)
+  ensures
+    && Inv(jm')
+    && I(jm') == I(jm).(inMemoryJournal := I(jm).inMemoryJournal + [je])
+  {
+    lenTimes8LeWeight(InMemoryJournal(jm));
+    lenTimes8LeWeight(InMemoryJournalFrozen(jm));
+
+    var idx := basic_mod(jm.start + jm.len1 + jm.len2);
+    var jm' := jm.(journalEntries := jm.journalEntries[idx as int := je])
+      .(len2 := jm.len2 + 1)
+      .(inMemoryWeight := jm.inMemoryWeight + WeightJournalEntry(je) as uint64 + (if jm.len2 == 0 then 8 else 0));
+
+    assert InMemoryJournal(jm')
+        == InMemoryJournal(jm) + [je] by { reveal_cyclicSlice(); }
+    assert InMemoryJournalFrozen(jm')
+        == InMemoryJournalFrozen(jm) by { reveal_cyclicSlice(); }
+    lemma_weight_append(InMemoryJournal(jm), je);
+    reveal_canAppend();
+
+    jm'
+  }
+
+  function {:opaque} isReplayEmpty(jm: JournalistModel) : (b: bool)
+  requires Inv(jm)
+  ensures b == (I(jm).replayJournal == [])
+  {
+    jm.replayIdx == |jm.replayJournal| as uint64
+  }
+}
