Versions/CompositeView_Refines_TSJMap.i.dfy
@@ -1,0 +1,189 @@
+include "CompositeView.i.dfy"
+include "../MapSpec/TSJMap.i.dfy"
+
+module CompositeView_Refines_TSJMap {
+  import CompositeView
+  import StatesViewMap
+  import TSJ = TSJMap
+  import opened Options
+  import opened Sequences
+  import opened Journal
+  import opened ViewOp
+  import MapSpec
+  import JournalView
+
+  function Ik(k: CompositeView.Constants) : TSJ.Constants
+  {
+    TSJ.Constants(k.tsm.k)
+  }
+
+  function I(k: CompositeView.Constants, s: CompositeView.Variables) : TSJ.Variables
+  requires CompositeView.Inv(k, s)
+  {
+    TSJ.Variables(
+      CompositeView.s1(s),
+      CompositeView.s2(s),
+      CompositeView.s3(s),
+      s.jc.j1,
+      s.jc.j2,
+      s.jc.j3,
+      s.jc.j_gamma,
+      s.jc.j_delta,
+      s.jc.syncReqs
+    )
+  }
+
+  lemma RefinesInit(k: CompositeView.Constants, s: CompositeView.Variables)
+    requires CompositeView.Init(k, s)
+    ensures CompositeView.Inv(k, s)
+    ensures TSJ.Init(Ik(k), I(k, s))
+  {
+    CompositeView.InitImpliesInv(k, s);
+  }
+
+  lemma SendPersistentLocRefines(k: CompositeView.Constants, s: CompositeView.Variables, s':CompositeView.Variables, uiop: UI.Op, vop: VOp)
+    requires CompositeView.Inv(k, s)
+    requires CompositeView.Inv(k, s')
+    requires CompositeView.NextStep(k, s, s', vop, uiop)
+    requires vop.SendPersistentLocOp?
+    ensures TSJ.Next(Ik(k), I(k, s), I(k, s'), uiop)
+  {
+    assert TSJ.NextStep(Ik(k), I(k, s), I(k, s'), uiop, TSJ.StutterStep);
+  }
+
+  lemma AdvanceRefines(k: CompositeView.Constants, s: CompositeView.Variables, s':CompositeView.Variables, uiop: UI.Op, vop: VOp)
+    requires CompositeView.Inv(k, s)
+    requires CompositeView.Inv(k, s')
+    requires CompositeView.NextStep(k, s, s', vop, uiop)
+    requires vop.AdvanceOp?
+    ensures TSJ.Next(Ik(k), I(k, s), I(k, s'), uiop)
+  {
+    if JournalView.Move3(k.jc, s.jc, s'.jc, vop) {
+      assert TSJ.NextStep(Ik(k), I(k, s), I(k, s'), uiop, TSJ.Move3Step);
+    } else if JournalView.Replay(k.jc, s.jc, s'.jc, vop) {
+      assert TSJ.NextStep(Ik(k), I(k, s), I(k, s'), uiop, TSJ.ReplayStep(vop.uiop));
+    }
+  }
+
+  lemma CrashRefines(k: CompositeView.Constants, s: CompositeView.Variables, s':CompositeView.Variables, uiop: UI.Op, vop: VOp)
+    requires CompositeView.Inv(k, s)
+    requires CompositeView.Inv(k, s')
+    requires CompositeView.NextStep(k, s, s', vop, uiop)
+    requires vop.CrashOp?
+    ensures TSJ.Next(Ik(k), I(k, s), I(k, s'), uiop)
+  {
+    assert TSJ.NextStep(Ik(k), I(k, s), I(k, s'), uiop, TSJ.CrashStep);
+  }
+
+  lemma FreezeRefines(k: CompositeView.Constants, s: CompositeView.Variables, s':CompositeView.Variables, uiop: UI.Op, vop: VOp)
+    requires CompositeView.Inv(k, s)
+    requires CompositeView.Inv(k, s')
+    requires CompositeView.NextStep(k, s, s', vop, uiop)
+    requires vop.FreezeOp?
+    ensures TSJ.Next(Ik(k), I(k, s), I(k, s'), uiop)
+  {
+    assert TSJ.NextStep(Ik(k), I(k, s), I(k, s'), uiop, TSJ.Move2to3Step);
+  }
+
+  lemma StatesInternalRefines(k: CompositeView.Constants, s: CompositeView.Variables, s':CompositeView.Variables, uiop: UI.Op, vop: VOp)
+    requires CompositeView.Inv(k, s)
+    requires CompositeView.Inv(k, s')
+    requires CompositeView.NextStep(k, s, s', vop, uiop)
+    requires vop.StatesInternalOp?
+    ensures TSJ.Next(Ik(k), I(k, s), I(k, s'), uiop)
+  {
+    assert TSJ.NextStep(Ik(k), I(k, s), I(k, s'), uiop, TSJ.StutterStep);
+  }
+
+  lemma JournalInternalRefines(k: CompositeView.Constants, s: CompositeView.Variables, s':CompositeView.Variables, uiop: UI.Op, vop: VOp)
+    requires CompositeView.Inv(k, s)
+    requires CompositeView.Inv(k, s')
+    requires CompositeView.NextStep(k, s, s', vop, uiop)
+    requires vop.JournalInternalOp?
+    ensures TSJ.Next(Ik(k), I(k, s), I(k, s'), uiop)
+  {
+    if JournalView.Move1to2(k.jc, s.jc, s'.jc, vop) {
+      assert TSJ.NextStep(Ik(k), I(k, s), I(k, s'), uiop, TSJ.Move1to2Step);
+    }
+    else if JournalView.ExtendLog1(k.jc, s.jc, s'.jc, vop) {
+      assert TSJ.NextStep(Ik(k), I(k, s), I(k, s'), uiop, TSJ.ExtendLog1Step);
+    }
+    else if JournalView.ExtendLog2(k.jc, s.jc, s'.jc, vop) {
+      assert TSJ.NextStep(Ik(k), I(k, s), I(k, s'), uiop, TSJ.ExtendLog2Step);
+    }
+    else if JournalView.Stutter(k.jc, s.jc, s'.jc, vop) {
+      assert TSJ.NextStep(Ik(k), I(k, s), I(k, s'), uiop, TSJ.StutterStep);
+    }
+  }
+
+  lemma SendFrozenLocRefines(k: CompositeView.Constants, s: CompositeView.Variables, s':CompositeView.Variables, uiop: UI.Op, vop: VOp)
+    requires CompositeView.Inv(k, s)
+    requires CompositeView.Inv(k, s')
+    requires CompositeView.NextStep(k, s, s', vop, uiop)
+    requires vop.SendFrozenLocOp?
+    ensures TSJ.Next(Ik(k), I(k, s), I(k, s'), uiop)
+  {
+    assert TSJ.NextStep(Ik(k), I(k, s), I(k, s'), uiop, TSJ.StutterStep);
+  }
+
+  lemma CleanUpRefines(k: CompositeView.Constants, s: CompositeView.Variables, s':CompositeView.Variables, uiop: UI.Op, vop: VOp)
+    requires CompositeView.Inv(k, s)
+    requires CompositeView.Inv(k, s')
+    requires CompositeView.NextStep(k, s, s', vop, uiop)
+    requires vop.CleanUpOp?
+    ensures TSJ.Next(Ik(k), I(k, s), I(k, s'), uiop)
+  {
+    assert TSJ.NextStep(Ik(k), I(k, s), I(k, s'), uiop, TSJ.StutterStep);
+  }
+
+  lemma PushSyncRefines(k: CompositeView.Constants, s: CompositeView.Variables, s':CompositeView.Variables, uiop: UI.Op, vop: VOp)
+    requires CompositeView.Inv(k, s)
+    requires CompositeView.Inv(k, s')
+    requires CompositeView.NextStep(k, s, s', vop, uiop)
+    requires vop.PushSyncOp?
+    ensures TSJ.Next(Ik(k), I(k, s), I(k, s'), uiop)
+  {
+    assert TSJ.NextStep(Ik(k), I(k, s), I(k, s'), uiop, TSJ.PushSyncStep(vop.id));
+  }
+
+  lemma PopSyncRefines(k: CompositeView.Constants, s: CompositeView.Variables, s':CompositeView.Variables, uiop: UI.Op, vop: VOp)
+    requires CompositeView.Inv(k, s)
+    requires CompositeView.Inv(k, s')
+    requires CompositeView.NextStep(k, s, s', vop, uiop)
+    requires vop.PopSyncOp?
+    ensures TSJ.Next(Ik(k), I(k, s), I(k, s'), uiop)
+  {
+    assert TSJ.NextStep(Ik(k), I(k, s), I(k, s'), uiop, TSJ.PopSyncStep(vop.id));
+  }
+
+  lemma RefinesNextStep(k: CompositeView.Constants, s: CompositeView.Variables, s':CompositeView.Variables, uiop: UI.Op, vop: VOp)
+    requires CompositeView.Inv(k, s)
+    requires CompositeView.Inv(k, s')
+    requires CompositeView.NextStep(k, s, s', vop, uiop)
+    ensures TSJ.Next(Ik(k), I(k, s), I(k, s'), uiop)
+  {
+    match vop {
+      case SendPersistentLocOp(loc) => { SendPersistentLocRefines(k, s, s', uiop, vop); }
+      case AdvanceOp(_, replay) => { AdvanceRefines(k, s, s', uiop, vop); }
+      case CrashOp => { CrashRefines(k, s, s', uiop, vop); }
+      case FreezeOp => { FreezeRefines(k, s, s', uiop, vop); }
+      case StatesInternalOp => { StatesInternalRefines(k, s, s', uiop, vop); }
+      case JournalInternalOp => { JournalInternalRefines(k, s, s', uiop, vop); }
+      case SendFrozenLocOp(loc) => { SendFrozenLocRefines(k, s, s', uiop, vop); }
+      case CleanUpOp => { CleanUpRefines(k, s, s', uiop, vop); }
+      case PushSyncOp(id) => { PushSyncRefines(k, s, s', uiop, vop); }
+      case PopSyncOp(id) => { PopSyncRefines(k, s, s', uiop, vop); }
+    }
+  }
+
+  lemma RefinesNext(k: CompositeView.Constants, s: CompositeView.Variables, s': CompositeView.Variables, uiop: UI.Op)
+    requires CompositeView.Inv(k, s)
+    requires CompositeView.Next(k, s, s', uiop)
+    ensures CompositeView.Inv(k, s')
+    ensures TSJ.Next(Ik(k), I(k, s), I(k, s'), uiop)
+  {
+    CompositeView.NextPreservesInv(k, s, s', uiop);
+    var vop :| CompositeView.NextStep(k, s, s', vop, uiop);
+    RefinesNextStep(k, s, s', uiop, vop);
+  }
+}
